Arithmetic/theories/Semantics.v
@@ -6,51 +6,50 @@ From Coq Require Import Strings.String.
 From Coq Require Import BinaryString.
 Open Scope Z_scope.
 
+Definition exp_sem_sig {T : Set} : Type := Env -> @_c_exp T -> 𝕍 -> Prop.
+Definition stmt_sem_sig {S T: Set} : Type  :=  @𝓕 S T -> @𝓟 S T-> Env -> @_c_statement S T ->  Env -> Prop.
+Definition Empty_exp_sem : @exp_sem_sig Empty_set := fun _ _ _ => False.
+Definition Empty_stmt_sem : @stmt_sem_sig Empty_set Empty_set := fun _ _ _ _ _ => False.
 
-Definition exp_sem_sig {T : Set} : Type := Ω -> 𝓜 -> @_c_exp T -> 𝕍 -> Prop.
-Definition stmt_sem_sig {S T: Set} : Type  :=  @𝓕 S T -> @𝓟 S T-> Ω -> 𝓜 -> @_c_statement S T ->  Ω -> 𝓜 -> Prop.
-Definition Empty_exp_sem : @exp_sem_sig Empty_set := fun _ _ _  _ => False.
-Definition Empty_stmt_sem : @stmt_sem_sig Empty_set Empty_set := fun _ _ _  _ _ _ _ => False.
 
-
-Declare Scope generic_sem_scope.
-Delimit Scope generic_sem_scope with gensem.
+Declare Scope generic_exp_sem_scope.
+Delimit Scope generic_exp_sem_scope with gesem.
 
 (* extensible expression semantic *)
-Inductive generic_exp_sem {T:Set} {ext_exp : @exp_sem_sig T} (env : Ω) (mem:𝓜): @_c_exp T -> 𝕍 -> Prop :=
-| C_E_Int (z:Z) irz : env ⋅ mem |= z => Int.mkMI z irz
+Inductive generic_exp_sem {T:Set} {ext_exp : @exp_sem_sig T} (ev:Env): @_c_exp T -> 𝕍 -> Prop :=
+| C_E_Int (z:Z) irz : ev |= z => VInt (z ⁱⁿᵗ irz)
 | C_E_Var (x:𝓥) z : 
-    (fst env) x = Some (Def (VInt z)) -> 
-    env ⋅ mem |=  (C_Id x C_Int) => z
+    ev x = Some (Def (VInt z)) -> 
+    ev |=  (C_Id x C_Int) => z
 | C_E_BinOpInt e e' (z z':Z) op z_ir z'_ir
     (H:Int.inRange (⋄ op z z')) :
-    env ⋅ mem |= e =>  (Int.mkMI z z_ir) ->
-    env ⋅ mem |= e' =>  (Int.mkMI z' z'_ir) ->
-    env ⋅ mem |=  BinOpInt e op e' => Int.mkMI ((⋄ op) z z') H
+    ev |= e =>  VInt (z ⁱⁿᵗ z_ir) ->
+    ev |= e' =>  VInt (z' ⁱⁿᵗ z'_ir) ->
+    ev |=  BinOpInt e op e' => VInt ((⋄ op) z z' ⁱⁿᵗ H)
 | C_E_BinOpTrue e e' (z z' : Z) z_ir z'_ir op :
-    env ⋅ mem |= e => (Int.mkMI z z_ir) ->
-    env ⋅ mem |= e' => (Int.mkMI z' z'_ir) ->
+    ev |= e => VInt (z ⁱⁿᵗ z_ir) ->
+    ev |= e' => VInt (z' ⁱⁿᵗ z'_ir) ->
     (◁ op) z z' = true ->
-    env ⋅ mem |= BinOpBool e op e'  => one
+    ev |= BinOpBool e op e' => VInt one
 | C_E_BinOpFalse e e' (z z' : Z) op z_ir z'_ir :
-    env ⋅ mem |= e => (Int.mkMI z z_ir) -> 
-    env ⋅ mem |= e' => (Int.mkMI z' z'_ir) -> 
+    ev |= e => VInt (z ⁱⁿᵗ z_ir) -> 
+    ev |= e' => VInt (z' ⁱⁿᵗ z'_ir) -> 
     ((◁ op) z z' = false ) ->
-    env ⋅ mem |= BinOpBool e op e' => zero
+    ev |= BinOpBool e op e' => VInt zero
 | C_Ext x v t: 
     (* variable must not be of type int (treated by C_E_Var) *)
     t <> C_Int ->
     
     (* variable must be bound and init *)
-    (fst env) x = Some (Def v) ->
+    ev x = Some (Def v) ->
 
 
     (* the external semantic can only add additional constraint, the result is always v *)
-    ext_exp env mem (C_Id x t) v ->
+    ext_exp ev (C_Id x t) v ->
 
-    env ⋅ mem |= (C_Id x t) => v
+    ev |= (C_Id x t) => v
 
-where  "Ω ⋅ M '|=' e => z" := (generic_exp_sem Ω M e z) : generic_sem_scope.
+where  "env '|=' e => z" := (generic_exp_sem env e z) : generic_exp_sem_scope.
 
 #[global] Hint Constructors generic_exp_sem  : rac_hint.
 
@@ -63,160 +62,167 @@ Definition c_exp_sem := @generic_exp_sem Empty_set Empty_exp_sem.
 
 Notation "Ω |= e => v"  := (c_exp_sem Ω ⊥ e v) : c_sem_scope.
 
-Inductive _gmp_exp_sem (env : Ω) (mem:𝓜) : gmp_exp -> 𝕍 -> Prop :=
+Inductive _gmp_exp_sem (ev:Env) : gmp_exp -> 𝕍 -> Prop :=
 | GMP_E_Var (x:𝓥) (l:location) (z:mpz_val) : 
-    (fst env) x = Some (Def (VMpz l)) -> 
-    mem l = Some z ->
-    _gmp_exp_sem env mem (C_Id x Mpz) (VMpz l)
+    ev x = Some (Def l) -> 
+    ev.(mstate) l = Some z ->
+    _gmp_exp_sem ev (C_Id x Mpz) (VMpz l)
 .
 
 #[global] Hint Constructors _gmp_exp_sem  : rac_hint.
 
-Declare Scope gmp_sem_scope.
-Delimit Scope gmp_sem_scope with gmpsem.
+Declare Scope gmp_exp_sem_scope.
+Delimit Scope gmp_exp_sem_scope with gmpesem.
 Definition gmp_exp_sem := @generic_exp_sem _gmp_t _gmp_exp_sem.
-Notation "Ω ⋅ M '|=' e => z" := (gmp_exp_sem Ω M e z) : gmp_sem_scope.
+Notation "ev '|=' e => z" := (gmp_exp_sem ev e z) : gmp_exp_sem_scope.
 
 Open Scope mini_c_scope.
+From RecordUpdate Require Import RecordUpdate.
+Import RecordSetNotations.
+
+Declare Scope generic_stmt_sem_scope.
+Delimit Scope generic_stmt_sem_scope with gssem.
 
 (* extensible statement semantic *)
-Inductive generic_stmt_sem {S T: Set} {ext_exp: @exp_sem_sig T} {ext_stmt: @stmt_sem_sig S T} (funs:@𝓕 S T) (procs: @𝓟 S T) (env:Ω) (mem:𝓜) : @_c_statement S T -> Ω -> 𝓜 -> Prop := 
-    | S_skip  :  (env ⋅ mem |= <{ skip }> => env ⋅ mem) funs procs
+Inductive generic_stmt_sem {S T: Set} {ext_exp: @exp_sem_sig T} {ext_stmt: @stmt_sem_sig S T} (funs:@𝓕 S T) (procs: @𝓟 S T) (ev:Env) : @_c_statement S T -> Env -> Prop := 
+    | S_skip  :  (ev |= <{ skip }> => ev) funs procs
     | S_Assign x z (e : @_c_exp T) : 
         (* must not be a compiler variable i.e. function return value *)
         is_comp_var x = false ->
 
-        type_of_value ((fst env) x) = Some C_Int ->
+        type_of_value (ev x) = Some C_Int ->
         (* value returned must be of same type*)
         type_of_value (Some z) = Some C_Int ->
 
-        @generic_exp_sem T ext_exp env mem e z -> 
-        (env ⋅ mem |= <{x = e}> => ((fst env){x\z},snd env) ⋅ mem) funs procs
+        @generic_exp_sem T ext_exp ev e z -> 
+        (ev |= <{x = e}> => (ev <| env ; vars ::= {{x\z}} |>)) funs procs
 
-    | S_IfTrue env' mem' z e s s' :
-        @generic_exp_sem T ext_exp env mem e z /\ ~ (z = zero) ->
-        (env ⋅ mem  |= s => env' ⋅ mem') funs procs ->
-        (env ⋅ mem  |= <{ if e s else s'}> => env' ⋅ mem') funs procs
+    | S_IfTrue ev' z e s s' :
+        @generic_exp_sem T ext_exp ev e z /\ ~ (z = VInt zero) ->
+        (ev  |= s => ev') funs procs ->
+        (ev  |= <{ if e s else s'}> => ev') funs procs
 
-    | S_IfFalse env' mem' e s s' :
-        @generic_exp_sem T ext_exp env mem e zero ->
-        (env ⋅ mem |= s' => env' ⋅ mem') funs procs ->
-        (env ⋅ mem |= <{ if e s else s'}> => env' ⋅ mem') funs procs
+    | S_IfFalse ev' e s s' :
+        @generic_exp_sem T ext_exp ev e (VInt zero) ->
+        (ev |= s' => ev') funs procs ->
+        (ev |= <{ if e s else s'}> => ev') funs procs
 
-    | S_While e s   env' mem' :
-        (env ⋅ mem |= <{ if e s ; while e s else skip }> =>  env' ⋅ mem') funs procs ->
-        (env ⋅ mem |= <{ while e s }> =>  env' ⋅ mem') funs procs
+    | S_While e s  ev' :
+        (ev |= <{ if e s ; while e s else skip }> => ev') funs procs ->
+        (ev |= <{ while e s }> => ev') funs procs
 
-    | S_Seq  env' mem' env'' mem'' s s' :
-        (env ⋅ mem |= s => env' ⋅ mem') funs procs ->
-        (env' ⋅ mem' |= s' => env'' ⋅ mem'') funs procs ->
-        (env ⋅ mem |= <{ s ; s' }> =>  env'' ⋅ mem'') funs procs
+    | S_Seq  ev' ev'' s s' :
+        (ev |= s => ev') funs procs ->
+        (ev' |= s' => ev'') funs procs ->
+        (ev |= <{ s ; s' }> =>  ev'') funs procs
 
-    | S_FCall f (b: @_c_statement S T) (env' : Ω) mem' c xargs eargs (zargs : 𝕍 ⃰ ) z : 
+    | S_FCall f (b: @_c_statement S T) ev' c xargs eargs (zargs : 𝕍 ⃰ ) z : 
         List.length xargs = List.length eargs ->
         funs f = Some (xargs,b) ->
-        List.Forall2 (@generic_exp_sem T ext_exp env mem) eargs zargs ->
-        (((p_map_addall ⊥ xargs zargs),⊥) ⋅ mem |= b => env' ⋅ mem') funs procs -> 
+        List.Forall2 (@generic_exp_sem T ext_exp ev) eargs zargs ->
+        (empty_env <| env ; vars ::= p_map_addall_back xargs zargs |> |= b => ev') funs procs -> 
         ~ List.In res_f (stmt_vars b) -> 
-        (fst env') res_f = Some (Def z) -> (* must be a defined value *)
-        (env ⋅ mem |= (FCall c f eargs) => ((fst env){c\Def z},(snd env)) ⋅ mem') funs procs
+        ev' res_f = Some (Def z) -> (* must be a defined value *)
+        (ev |= (FCall c f eargs) => ev <| env ; vars ::= {{c\Def z}} |> <| mstate := ev' |>) funs procs
 
-    | S_PCall p b (env' : Ω) mem' xargs eargs zargs : 
+    | S_PCall p b ev' xargs eargs zargs : 
         List.length xargs = List.length eargs ->
         procs p = Some (xargs,b) ->
-        List.Forall2 (@generic_exp_sem T ext_exp env mem) eargs zargs ->
-        (((p_map_addall ⊥ xargs zargs),⊥) ⋅ mem |= b => env'⋅ mem') funs procs ->
-        (env ⋅ mem |= PCall p eargs => env ⋅ mem') funs procs
+        List.Forall2 (@generic_exp_sem T ext_exp ev) eargs zargs ->
+        (empty_env <| env ; vars ::= p_map_addall_back xargs zargs |> |= b => ev') funs procs -> 
+        (ev |= PCall p eargs => ev <| mstate := ev' |>) funs procs
 
     | S_Return e z : 
         (* not allowed to return an unassigned value *)
-        @generic_exp_sem T ext_exp env mem e (Def z) ->
-        (env ⋅ mem |= <{ return e }> =>  ((fst env){res_f\Def z},snd env)⋅ mem) funs procs
+        @generic_exp_sem T ext_exp ev e (Def z) ->
+        (ev |= <{ return e }> => ev <| env ; vars ::= {{res_f\Def z}} |>) funs procs
 
     | S_PAssert  e z :
-        @generic_exp_sem T ext_exp env mem e z -> z <>  zero ->
-        (env ⋅ mem |= <{ assert e }> => env ⋅ mem) funs procs
+        @generic_exp_sem T ext_exp ev e z -> z <> VInt zero ->
+        (ev |= <{ assert e }> => ev) funs procs
 
-    | S_ExtSem s env' mem' : 
+    | S_ExtSem s ev' :  
         (* only S_Ext constructor allowed to use external semantic*)
-        ext_stmt funs procs env mem (S_Ext s) env' mem' 
-        -> (env ⋅ mem |= (S_Ext s) => env' ⋅ mem') funs procs
+        ext_stmt funs procs ev (S_Ext s) ev' 
+        -> (ev |= (S_Ext s) => ev') funs procs
     
-    where "Ω ⋅ M |= s => Ω' ⋅ M'"  := (fun funs procs => generic_stmt_sem funs procs Ω M s Ω' M') : generic_sem_scope.
+    where "env |= s => env'"  := (fun funs procs => generic_stmt_sem funs procs env s env') : generic_stmt_sem_scope.
     
 #[global] Hint Constructors generic_stmt_sem  : rac_hint.
 
 
-Declare Scope c_sem_scope.
+(* Declare Scope c_sem_scope.
 Delimit Scope c_sem_scope with csem. 
 Definition c_stmt_sem := @generic_stmt_sem Empty_set Empty_set Empty_exp_sem Empty_stmt_sem.
-Notation "Ω ⋅ M |= s => Ω' ⋅ M'"  := (c_stmt_sem Ω M s Ω' M') : c_sem_scope.
+Notation "ev |= s => ev'"  := (c_stmt_sem ev s ev') : c_sem_scope. *)
 
 
 
 Definition c_decl_sem (env env':Ω) (mem mem':𝓜) d : Prop := 
         forall x t u,
-        (fst env) x  = None -> 
+        env x  = None -> 
         (Uτ u) = Some t ->
-        d = C_Decl t x -> env' = ((fst env){x\u},snd env) /\ mem = mem'.
+        d = C_Decl t x -> env' = env <| vars ::= {{x\u}} |> /\ mem = mem'.
         
 
 
-Open Scope gmp_sem_scope.
+Open Scope gmp_exp_sem_scope.
 Open Scope mini_gmp_scope.
+Declare Scope gmp_stmt_sem_scope.
+Delimit Scope gmp_stmt_sem_scope with gmpssem.
 
-Inductive _gmp_stmt_sem { S T : Set }(funs : @𝓕 S T) (procs : @𝓟 S T) (env:Ω) (mem:𝓜) : gmp_statement -> Ω -> 𝓜 -> Prop := 
+Inductive _gmp_stmt_sem { S T : Set }(funs : @𝓕 S T) (procs : @𝓟 S T) (ev:Env) : gmp_statement -> Env -> Prop := 
     | S_init x (l:location):
-        (forall v, (fst env) v <> Some (Def (VMpz (Some l)))) ->
-        (exists n, (fst env) x = Some (Undef (UMpz n)))%type ->
-        (env ⋅ mem |= <init(x)> => ((fst env){x\Def (VMpz (Some l))}, snd env) ⋅ mem{l\Defined 0}) funs procs
+        (forall v, ev v <> Some (Def (VMpz (Some l)))) ->
+        (exists n, ev x = Some (Undef (UMpz n)))%type ->
+        (ev |= <(init(x))> => ev <| env ; vars ::= {{x\Def (VMpz (Some l))}} |> <| mstate ::= {{l\Defined 0}} |>) funs procs
     
     | S_clear x a u:   
-        (fst env) x = Some (Def (VMpz (Some a))) ->   
-        (env ⋅ mem |= <cl(x)> => ((fst env){x\(Def (VMpz None))}, snd env) ⋅ mem{a\Undefined u}) funs procs
+        ev x = Some (Def (VMpz (Some a))) ->   
+        (ev |= <(cl(x))> => ev <| env ; vars ::= {{x\(Def (VMpz None))}} |> <| mstate ::= {{a\Undefined u}} |>) funs procs
 
     | S_set_i x y z a :  
-        (fst env) x = Some (Def (VMpz (Some a))) ->
-        env ⋅ mem |= y => VInt z ->
-        (env ⋅ mem |= <set_i(x,y)> => env ⋅ mem{a\Defined (z ̇)}) funs procs
+        ev x = Some (Def (VMpz (Some a))) ->
+        (ev |= y => VInt z)%gmpesem ->
+        (ev |= <(set_i(x,y))> => ev <| mstate ::= {{a\Defined (z ̇)}} |>) funs procs
 
     | S_set_z x y z (a n : location) :  
-        (fst env) x = Some (Def (VMpz a)) ->
-        (fst env) y = Some (Def (VMpz n)) ->
-        mem n = Some z ->
-        (env ⋅ mem |= <set_z(x,y)> => env ⋅ mem{a\z}) funs procs 
+        ev x = Some (Def (VMpz a)) ->
+        ev y = Some (Def (VMpz n)) ->
+        ev.(mstate) n = Some z ->
+        (ev |= <(set_z(x,y))> => ev <| mstate ::= {{a\z}} |>) funs procs 
 
     | S_get_int x (y:id) z v (ir:Int.inRange z) :
-        env ⋅ mem |= C_Id y Mpz => VMpz (Some v) ->
-        mem v = Some (Defined z) -> 
-        (env ⋅ mem |= <x = get_int(y)> => ((fst env){x\z ⁱⁿᵗ ir : 𝕍},(snd env)) ⋅ mem) funs procs
+        (ev |= C_Id y Mpz => VMpz (Some v))%gmpesem ->
+        ev.(mstate) v = Some (Defined z) -> 
+        (ev |= <(x = get_int(y))> => ev <| env ; vars ::= {{x\VInt (z ⁱⁿᵗ ir) : 𝕍}} |>) funs procs
 
     | S_set_s s x z a :
-        (fst env) x = Some (Def (VMpz (Some a))) ->
+        ev x = Some (Def (VMpz (Some a))) ->
         BinaryString.to_Z s = z ->
-        (env ⋅ mem |= <set_s(x,s)> => env ⋅ mem{a\Defined z}) funs procs
+        (ev |= <(set_s(x,s))> => ev <| mstate ::= {{a\Defined z}} |> ) funs procs
 
     | S_cmp c x (vx vy :location) lx y ly (b:𝕍):
-        env ⋅ mem |= C_Id x Mpz => vx ->
-        env ⋅ mem |= C_Id y Mpz => vy ->
-        mem vx = Some (Defined lx) ->
-        mem vy = Some (Defined ly) ->
+        (ev |= C_Id x Mpz => vx)%gmpesem ->
+        (ev |= C_Id y Mpz => vy)%gmpesem ->
+        ev.(mstate) vx = Some (Defined lx) ->
+        ev.(mstate) vy = Some (Defined ly) ->
         (
-            (Z.gt lx ly <-> b = one) /\
-            (Z.lt lx ly <-> b = sub_one) /\
-            (Z.eq lx ly <-> b = zero)
+            (Z.gt lx ly <-> b = VInt one) /\
+            (Z.lt lx ly <-> b = VInt sub_one) /\
+            (Z.eq lx ly <-> b = VInt zero)
         ) ->
-        (env ⋅ mem |= <c = cmp(x,y)> => ((fst env){c\b}, snd env) ⋅ mem) funs procs
+        (ev |= <(c = cmp(x,y))> => ev <| env ; vars ::= {{c\b}} |>) funs procs
     
     | S_op bop r lr x y (vx vy : location) z1 z2 :
-        env ⋅ mem |= C_Id x Mpz => vx ->
-        mem vx = Some (Defined z1) -> 
-        env ⋅ mem |= C_Id y Mpz =>  vy ->
-        mem vy = Some (Defined z2) -> 
-        (fst env) r = Some (Def (VMpz (Some lr))) ->
-        (env ⋅ mem |= op bop r x y => env ⋅ mem{lr\Defined (⋄ (□ bop) z1 z2) }) funs procs
+        (ev |= C_Id x Mpz => vx)%gmpesem ->
+        ev.(mstate) vx = Some (Defined z1) -> 
+        (ev |= C_Id y Mpz =>  vy)%gmpesem ->
+        ev.(mstate) vy = Some (Defined z2) -> 
+        ev r = Some (Def (VMpz (Some lr))) ->
+        (ev |= op bop r x y => ev <| mstate ::= {{lr\Defined (⋄ (□ bop) z1 z2) }} |>) funs procs
 
-where "Ω ⋅ M |= s => Ω' ⋅ M'"  := (fun funs procs => _gmp_stmt_sem funs procs Ω M s Ω' M') : gmp_sem_scope.
+where "ev |= s => ev'"  := (fun funs procs => _gmp_stmt_sem funs procs ev s ev') : gmp_stmt_sem_scope.
 
 #[global] Hint Constructors _gmp_stmt_sem  : rac_hint.
 
@@ -226,63 +232,63 @@ Definition gmp_stmt_sem := @generic_stmt_sem _gmp_statement _gmp_t _gmp_exp_sem 
 Notation "Ω ⋅ M |= s => Ω' ⋅ M'"  := (fun funs procs => gmp_stmt_sem funs procs Ω M s Ω' M') : gmp_sem_scope. 
  *)
 
-Inductive fsl_term_sem (env:Ω) : ℨ -> Z -> Prop :=
-| FSL_E_Int z : fsl_term_sem env (T_Z z) z 
-| FSL_E_LVar x z : (snd env) x = Some z -> fsl_term_sem env (T_Id x) z
+Inductive fsl_term_sem (ev:Env) : ℨ -> Z -> Prop :=
+| FSL_E_Int z : fsl_term_sem ev (T_Z z) z 
+| FSL_E_LVar x z : ev.(binds) x = Some z -> fsl_term_sem ev (T_Id x) z
 | FSL_E_Var x v : 
-    (fst env) v = Some (Def (VInt x)) ->  
-    fsl_term_sem env (T_Id v) x ̇
+    ev v = Some (Def (VInt x)) ->  
+    fsl_term_sem ev (T_Id v) x ̇
 
 | FSL_E_BinOpInt t t' z zint z' z'int op :  
-    fsl_term_sem env t z ->
-    fsl_term_sem env t' z' ->
+    fsl_term_sem ev t z ->
+    fsl_term_sem ev t' z' ->
     ~ (op = FSL_Div /\ z = 0)%type ->
-    fsl_term_sem env (T_BinOp t op t') ((fsl_binop_int_model op) zint z'int)
+    fsl_term_sem ev (T_BinOp t op t') ((fsl_binop_int_model op) zint z'int)
 
 | FSL_E_CondTrue p t z t':
-    fsl_pred_sem env p BTrue ->
-    fsl_term_sem env t z ->
-    fsl_term_sem env (T_Cond p t t') z
+    fsl_pred_sem ev p BTrue ->
+    fsl_term_sem ev t z ->
+    fsl_term_sem ev (T_Cond p t t') z
 
 | FSL_E_CondFalse p t t' z':
-    fsl_pred_sem env p BFalse ->
-    fsl_term_sem env t' z' ->
-    fsl_term_sem env (T_Cond p t t') z'
+    fsl_pred_sem ev p BFalse ->
+    fsl_term_sem ev t' z' ->
+    fsl_term_sem ev (T_Cond p t t') z'
 
     with 
 
-fsl_pred_sem (env:Ω) :  𝔅 -> 𝔹 -> Prop :=
-| FP_True : fsl_pred_sem env P_True BTrue
-| FP_False : fsl_pred_sem env P_False BFalse
+fsl_pred_sem (ev:Env) :  𝔅 -> 𝔹 -> Prop :=
+| FP_True : fsl_pred_sem ev P_True BTrue
+| FP_False : fsl_pred_sem ev P_False BFalse
 
 | FP_BinOpTrue t t' z z' (op:fsl_binop_bool): 
-    fsl_term_sem env t z ->
-    fsl_term_sem env t' z' ->
+    fsl_term_sem ev t z ->
+    fsl_term_sem ev t' z' ->
     (fsl_binop_bool_model op) z z' ->
-    fsl_pred_sem env (P_BinOp t op t) BTrue
+    fsl_pred_sem ev (P_BinOp t op t) BTrue
 
 | FP_BinOpFalse t t' z z' (op:fsl_binop_bool): 
-    fsl_term_sem env t z ->
-    fsl_term_sem env t' z' ->
+    fsl_term_sem ev t z ->
+    fsl_term_sem ev t' z' ->
     ~ (fsl_binop_bool_model op) z z' ->
-    fsl_pred_sem env (P_BinOp t op t) BFalse
+    fsl_pred_sem ev (P_BinOp t op t) BFalse
 
 | FP_NotTrue p : 
-    fsl_pred_sem env p BTrue ->
-    fsl_pred_sem env (Not p) BFalse
+    fsl_pred_sem ev p BTrue ->
+    fsl_pred_sem ev (Not p) BFalse
 
 | FP_NotFalse p : 
-    fsl_pred_sem env p BFalse ->
-    fsl_pred_sem env (Not p) BTrue 
+    fsl_pred_sem ev p BFalse ->
+    fsl_pred_sem ev (Not p) BTrue 
 
 | FP_DisjLeftTrue p p' : 
-    fsl_pred_sem env p BTrue ->
-    fsl_pred_sem env (Disj p p') BTrue 
+    fsl_pred_sem ev p BTrue ->
+    fsl_pred_sem ev (Disj p p') BTrue 
 
 | FP_DisjLeftFalse p p' z : 
-    fsl_pred_sem env p BFalse ->
-    fsl_pred_sem env p' z ->
-    fsl_pred_sem env (Disj p p') z
+    fsl_pred_sem ev p BFalse ->
+    fsl_pred_sem ev p' z ->
+    fsl_pred_sem ev (Disj p p') z
 .
 
 #[global] Hint Constructors fsl_term_sem : rac_hint.
@@ -291,19 +297,19 @@ fsl_pred_sem (env:Ω) :  𝔅 -> 𝔹 -> Prop :=
 Declare Scope fsl_sem_scope.
 Delimit Scope fsl_sem_scope with fslsem.
 
-Notation "Ω '|=' t => v" := (fsl_term_sem Ω t v) : fsl_sem_scope.
+(* Notation "Ω '|=' t => v" := (fsl_term_sem Ω t v) : fsl_sem_scope. *)
 
-Inductive _fsl_assert_sem { S T : Set } (funs : @𝓕 S T) (procs : @𝓟 S T) (env : Ω) (mem:𝓜) : fsl_statement -> Ω -> 𝓜 -> Prop :=
+Inductive _fsl_assert_sem { S T : Set } (funs : @𝓕 S T) (procs : @𝓟 S T) (ev:Env) : fsl_statement -> Env -> Prop :=
 | FSL_Assert (p:𝔅) : 
-    fsl_pred_sem env p BTrue ->
-    _fsl_assert_sem funs procs env mem (LAssert p) env mem
+    fsl_pred_sem ev p BTrue ->
+    _fsl_assert_sem funs procs ev (LAssert p) ev
 .
 
 #[global] Hint Constructors _fsl_assert_sem : rac_hint.
 
 
 Definition fsl_stmt_sem := @generic_stmt_sem _fsl_statement _gmp_t gmp_exp_sem _fsl_assert_sem.
-Notation "Ω ⋅ M |= s => Ω' ⋅ M'"  := (fun funs procs => fsl_stmt_sem funs procs Ω M s Ω' M') : fsl_sem_scope. 
+Notation "ev |= s => ev'"  := (fun funs procs => fsl_stmt_sem funs procs ev s ev') : fsl_sem_scope. 
 
 
 
@@ -311,14 +317,14 @@ Notation "Ω ⋅ M |= s => Ω' ⋅ M'"  := (fun funs procs => fsl_stmt_sem funs 
 
 
 Declare Scope macro_sem_scope.
-Inductive macro_sem (env : Ω) (mem:𝓜) (e:gmp_exp): Z -> Prop :=
+Inductive macro_sem (ev:Env) (e:gmp_exp): Z -> Prop :=
 | M_Int x :  
-    gmp_exp_sem env mem e (VInt x) ->
-    env ⋅ mem |= e ⇝ x ̇
+    gmp_exp_sem ev e (VInt x) ->
+    ev |= e ⇝ x ̇
 | M_Mpz l z : 
-    gmp_exp_sem env mem e (VMpz (Some l)) ->
-    mem l = Some (Defined z) ->
-    env ⋅ mem |= e ⇝ z
-where "Ω ⋅ M '|=' e ⇝ z" := (macro_sem Ω M e z) : macro_sem_scope.
+    gmp_exp_sem ev e (VMpz (Some l)) ->
+    ev.(mstate) l = Some (Defined z) ->
+    ev |= e ⇝ z
+where "ev '|=' e ⇝ z" := (macro_sem ev e z) : macro_sem_scope.
 
 #[global] Hint Constructors macro_sem : rac_hint.
