Arithmetic/theories/Theorems.v
@@ -9,32 +9,34 @@ From Coq Require Import ZArith.ZArith.
 Open Scope utils_scope.
 Open Scope definition_scope.
 
+From RecordUpdate Require Import RecordUpdate.
+Import RecordSetNotations.
 
 (* Properties of the semantics *)
 
 
 
-Definition _no_env_mpz_aliasing (env : Ω) : Prop := 
+Definition _no_env_mpz_aliasing (ev : Ω) : Prop := 
     forall v v' l l', 
     v <> v' ->
-    (fst env) v = Some (Def (VMpz (Some l)))  ->
-    (fst env) v' = Some (Def (VMpz (Some l'))) -> 
+    ev v = Some (Def (VMpz (Some l)))  ->
+    ev v' = Some (Def (VMpz (Some l'))) -> 
     l <> l'.
 
 Definition _no_mem_aliasing {S T : Set} (stmt_sem : @stmt_sem_sig S T)  : Prop := 
-    forall (exp_sem:@exp_sem_sig T) funs procs env mem s env' mem', 
-    _no_env_mpz_aliasing env 
-    -> stmt_sem funs procs env mem s env' mem' 
-    -> _no_env_mpz_aliasing env'.
+    forall (exp_sem:@exp_sem_sig T) funs procs (ev:Env) s (ev':Env), 
+    _no_env_mpz_aliasing ev
+    -> stmt_sem funs procs ev s ev' 
+    -> _no_env_mpz_aliasing ev'.
 
 
 Fact _no_mem_aliasing_gmp : _no_mem_aliasing _gmp_stmt_sem.
 Proof with auto with rac_hint.
-    intros exp_sem funs procs env mem s env' mem' Hnoalias H. induction H
+    intros exp_sem funs procs ev s ev' Hnoalias H. induction H
     ; auto ;  try (rename v into l1) ;
-    intros v v' ll l' Hvv' Hl Hl' leq ; subst ; simpl in *.
+    intros v v' ll l' Hvv' Hl Hl' leq ; subst ; autounfold with rac_hint in * ; simpl in *.
     - destruct (eq_dec x v).
-        + subst. rewrite p_map_same in Hl. rewrite p_map_not_same in Hl'... inversion Hl. 
+        + subst. autounfold with rac_hint in *. rewrite p_map_same in Hl. rewrite p_map_not_same in Hl'... inversion Hl. 
             subst. now destruct H with v'.
         + rewrite p_map_not_same in Hl... destruct (eq_dec x v').
             * subst. rewrite p_map_same in Hl'. inversion Hl'. subst. now destruct H with v.
@@ -105,13 +107,13 @@ Proof with auto with rac_hint.
 Admitted. *)
 
 Fact eq_env_partial_order :  forall e e' v z, (e ⊑ e')%env ->  
-    (fst e) v = Some (Def z) -> (fst e') v = Some (Def z).
+    e v = Some (Def z) -> e' v = Some (Def z).
 Proof.
     intros e e' v z Hrel He. destruct Hrel with v; congruence.
 Qed.
 
-Fact sym_env_cond : forall env env', 
-(forall v, (dom (fst env) - dom (fst env')) v ) -> (env ⊑ env')%env -> (env' ⊑ env)%env.
+Fact sym_env_cond : forall (env env' : Ω), 
+(forall v, (dom env - dom env') v ) -> (env ⊑ env')%env -> (env' ⊑ env)%env.
 
 Proof.
     intros env env' H rel v ; destruct H with v as [Hin Hnotin] ; destruct Hnotin ; destruct rel with v.
@@ -126,10 +128,10 @@ Proof.
     - destruct Hin. destruct env. simpl in *. congruence.
 Qed.
 
-Corollary sym_env_cond_mem : forall (env : Ω) env' mem mem', 
-(forall v, (dom (fst env) - dom (fst env')) v ) -> (env,mem) ⊑ (env',mem') ->  (env',mem) ⊑ (env,mem').
+Corollary sym_env_cond_mem : forall (ev ev' : Env), 
+(forall v, (dom ev - dom ev') v ) -> (ev ⊑ ev')%envmem ->  (mkEnv ev' ev ⊑ mkEnv ev ev')%envmem.
 Proof.
-    intros. split. apply sym_env_cond ; easy. now destruct H0.
+    intros [env mem]. split. now apply sym_env_cond. now destruct H0.
 Qed.
 
 
@@ -137,11 +139,11 @@ Qed.
 
 Corollary eq_env_partial_order_add :  forall (e e' :Ω) v v' z z',  (e ⊑ e')%env ->  
     v <> v' ->
-    (fst e) v = Some (Def z) -> ((fst e'){v'\z'}) v = Some (Def z).
+    e v = Some (Def z) -> (e'{v'\z'}) v = Some (Def z).
 Proof.
     intros [v l] [v' l'] var var' z z' Hrel Hneq H. 
-    pose proof (eq_env_partial_order (v,l) (v',l') var z Hrel H).
-    pose proof (p_map_not_same v' var var' z' Hneq). simpl in *. congruence.
+    pose proof (eq_env_partial_order {|vars:=v;binds:=l|} {|vars:=v';binds:=l'|} var z Hrel H).
+    pose proof (p_map_not_same {| vars := v'; binds := l' |} var var' z' Hneq). congruence.
 Qed.
 
 
@@ -158,7 +160,7 @@ Qed.
 
 Fact env_partial_order_add : forall Ω₀ Ω₀', (Ω₀ ⊑ Ω₀')%env -> 
     (forall var' z, 
-    ( ( (fst Ω₀) {var' \ z}, snd Ω₀) ) ⊑  ( ((fst (Ω₀')) {var' \ z}, snd Ω₀') )
+    Ω₀ <| vars ::= fun x => x{var' \ z} |> ⊑  Ω₀' <| vars ::= fun x => x{var' \ z} |>
     )%env.
 Proof with auto with rac_hint.
     intros [v l][v' l'] H x z var. destruct (string_dec x var) as [Heq|Hneq].
@@ -172,28 +174,31 @@ Proof with auto with rac_hint.
 
     - apply not_eq_sym in Hneq. epose proof (p_map_not_same v var x ?[z] Hneq) as H0. simpl. remember (v var) as res. destruct res as [z'|].
         * destruct z'.
-            + destruct v0.
-                ++ apply EsameInt with n ; simpl.
-                    +++ apply H0.
-                    +++ apply p_map_not_same_eq in H0... epose proof (eq_env_partial_order_add  _ _ _ _ _ _ H). 
+            + { 
+                destruct v0.
+                - apply EsameInt with n ; simpl.
+                    + apply H0.
+                    + apply p_map_not_same_eq in H0... epose proof (eq_env_partial_order_add  _ _ _ _ _ _ H). 
                         now apply H1.
-                ++ apply EsameMpz with l0; simpl... epose proof (eq_env_partial_order_add  _ _ _ _ _ _ H).
+                - apply EsameMpz with l0; simpl... epose proof (eq_env_partial_order_add  _ _ _ _ _ _ H).
                     symmetry in Heqres. specialize (H1 Hneq Heqres). simpl in H1. apply H1.
+            }
 
-            + destruct uv.
-                ++ eapply EundefInt ;subst ;simpl.
-                    +++ apply H0.
-                    +++ destruct H with var ; pose proof (p_map_not_same_eq v' var x z) as Hres; simpl in *; try congruence.
+            + {
+                destruct uv.
+                - eapply EundefInt ;subst ;simpl. 
+                    + apply H0.
+                    + destruct H with var ; pose proof (p_map_not_same_eq v' var x z) as Hres; simpl in *; try congruence.
                         destruct H2.
-                    ++++ specialize (Hres  (Some (Undef (UInt n))) Hneq). left. apply Hres. congruence.
-                    ++++ destruct H2 as [x0]. specialize (Hres  (Some (Def (VInt x0))) Hneq). right. exists x0. now apply Hres.
-
-                ++ eapply EundefMpz ; subst ; simpl.
-                    +++ apply H0.
-                    +++ destruct H with var ; pose proof (p_map_not_same_eq v' var x z) as Hres; simpl in * ; try congruence.
+                        * specialize (Hres  (Some (Undef (UInt n))) Hneq). left. apply Hres. congruence.
+                        * destruct H2 as [x0]. specialize (Hres  (Some (Def (VInt x0))) Hneq). right. exists x0. now apply Hres.
+                - eapply EundefMpz ; subst ; simpl.
+                    + apply H0.
+                    + destruct H with var ; pose proof (p_map_not_same_eq v' var x z) as Hres; simpl in * ; try congruence.
                         destruct H2.
-                        ++++ specialize (Hres  (Some (Undef (UMpz l0))) Hneq). left.  apply Hres. congruence.
-                        ++++ destruct H2 as [l0']. specialize (Hres  (Some (Def (VMpz l0'))) Hneq). right. exists l0'. now apply Hres.
+                        * specialize (Hres  (Some (Undef (UMpz l0))) Hneq). left.  apply Hres. congruence.
+                        * destruct H2 as [l0']. specialize (Hres  (Some (Def (VMpz l0'))) Hneq). right. exists l0'. now apply Hres.
+            }
         * now apply Enone.
 Qed.
 
@@ -206,21 +211,19 @@ Proof.
 Qed.
 
 
-Fact env_same_ty : forall  (Ω Ω' : Ω) v t, (Ω ⊑ Ω')%env -> t <> None -> type_of_value (fst Ω v) = t -> type_of_value (fst Ω' v) = t.
+Fact env_same_ty : forall  (Ω Ω' : Ω) v t, (Ω ⊑ Ω')%env -> t <> None -> type_of_value (Ω v) = t -> type_of_value (Ω' v) = t.
 Proof.
     intros. 
-    match goal with | IncRel : (_ ⊑ _)%env |- _ =>  destruct IncRel with v ; subst end ;
+    match goal with | IncRel : (_ ⊑ _)%env |- _ =>  destruct IncRel with v ; subst end;
     match goal with 
-    | L : fst Ω v = _,  R : fst Ω' v = _  |- _ => now rewrite L,R 
-    | L : fst Ω v = _,  R : fst Ω' v = _ \/ _ |- _ => destruct R as [SomeUInt | [ x Some_n ]]; [now rewrite L,SomeUInt | now rewrite L,Some_n] 
+    | L : apply_env Ω v = _,  R : apply_env Ω' v = _  |- _ => now rewrite L,R 
+    | L : apply_env Ω v = _,  R : apply_env Ω' v = _ \/ _ |- _ => destruct R as [SomeUInt | [ x Some_n ]]; [now rewrite L,SomeUInt | now rewrite L,Some_n] 
     | L : _ = None,  Contra : _ <> None |- _ =>  now rewrite L in Contra
     end.
 Qed.
 
-Open Scope generic_sem_scope.
-
 Definition _determinist_exp_eval {T : Set} (exp_sem : @exp_sem_sig T) : Prop := 
-    forall e env mem v,  exp_sem env mem e v ->  (forall v', exp_sem env mem e v' -> v = v')
+    forall e ev v,  exp_sem ev e v ->  (forall v', exp_sem ev e v' -> v = v')
 .
 
 Fact determinist_exp_eval {T : Set}: 
@@ -228,14 +231,14 @@ forall ext_exp_sem, _determinist_exp_eval ext_exp_sem -> _determinist_exp_eval (
 Proof.
     intros ext_exp_sem ext_inj. unfold _determinist_exp_eval. intros e. induction e ; intros ; inversion H ; inversion H0 ; subst ; try easy.
     5,6:
-        apply IHe1 with (v:=(z ⁱⁿᵗ z_ir)) (v':=(z0 ⁱⁿᵗ z_ir0)) in H11 ; [|assumption] ; injection H11 as eqz ;
-        apply IHe2 with (v:=(z' ⁱⁿᵗ z'_ir)) (v':=(z'0 ⁱⁿᵗ z'_ir0)) in H13; [|assumption] ;  injection H13 as eqz' ; subst ; now rewrite H14 in H7.
-    - f_equal. now apply Int.mi_eq. 
+        apply IHe1 with (v:=VInt (z ⁱⁿᵗ z_ir)) (v':=VInt (z0 ⁱⁿᵗ z_ir0)) in H11 ; [|assumption] ; injection H11 as eqz ;
+        apply IHe2 with (v:=VInt (z' ⁱⁿᵗ z'_ir)) (v':= VInt (z'0 ⁱⁿᵗ z'_ir0)) in H13; [|assumption] ;  injection H13 as eqz' ; subst ; now rewrite H14 in H7.
+    - f_equal. f_equal. now apply Int.mi_eq. 
     - congruence.
     - destruct ty. easy. 1,2: apply ext_inj in H6 ; now apply H6 in H12.
-    - f_equal. apply Int.mi_eq. simpl. f_equal.
-        + apply IHe1 with (v:=(z ⁱⁿᵗ z_ir)) (v':=(z0 ⁱⁿᵗ z_ir0)) in H13; [|assumption]. now injection H13. 
-        + apply IHe2 with (v:=(z' ⁱⁿᵗ z'_ir)) (v':=(z'0 ⁱⁿᵗ z'_ir0)) in H14; [|assumption]. now injection H14.
+    - f_equal. f_equal. apply Int.mi_eq. simpl. f_equal.
+        + apply IHe1 with (v:=VInt (z ⁱⁿᵗ z_ir)) (v':= VInt (z0 ⁱⁿᵗ z_ir0)) in H13; [|assumption]. now injection H13. 
+        + apply IHe2 with (v:=VInt (z' ⁱⁿᵗ z'_ir)) (v':=VInt (z'0 ⁱⁿᵗ z'_ir0)) in H14; [|assumption]. now injection H14.
 Qed.
 
 Fact _determinist_c_exp_eval : _determinist_exp_eval Empty_exp_sem.
@@ -245,20 +248,20 @@ Definition determinist_c_exp_eval := determinist_exp_eval Empty_exp_sem _determi
 
 Fact _determinist_gmp_exp_eval :  _determinist_exp_eval _gmp_exp_sem.
 Proof.
-    unfold _determinist_exp_eval. intros e. induction e ; intros env mem v H v' H0. inversion H ; inversion H0 ; subst.
-    - inversion H ; inversion H0 ; subst ; try easy. congruence. 
+    unfold _determinist_exp_eval. intros e. induction e ; intros ev v H v' H0. inversion H ; inversion H0 ; subst.
+    - inversion H ; inversion H0 ; subst ; try easy. rewrite H3 in H8.  repeat f_equal. now injection H8. 
     - inversion H.
     - inversion H.
 Qed.
 
 Definition determinist_gmp_exp_eval := determinist_exp_eval _gmp_exp_sem _determinist_gmp_exp_eval.
 
-Fact Forall2_same_zargs { T : Set} : forall env mem eargs zargs zargs0  exp_sem, 
+Fact Forall2_same_zargs { T : Set} : forall ev eargs zargs zargs0  exp_sem, 
     _determinist_exp_eval exp_sem
-    -> List.Forall2 (@generic_exp_sem T exp_sem env mem) eargs zargs 
-    -> List.Forall2 (@generic_exp_sem T exp_sem env mem) eargs zargs0 -> zargs = zargs0.
+    -> List.Forall2 (@generic_exp_sem T exp_sem ev) eargs zargs 
+    -> List.Forall2 (@generic_exp_sem T exp_sem ev) eargs zargs0 -> zargs = zargs0.
 Proof.
-    intros env mem eargs zargs zargs0 exp H  Hderiv. generalize dependent zargs0. induction Hderiv ; intros zargs0 H1.
+    intros ev eargs zargs zargs0 exp H  Hderiv. generalize dependent zargs0. induction Hderiv ; intros zargs0 H1.
     - now inversion H1.
     - destruct zargs0. inversion H1. apply List.Forall2_cons_iff in H1 as [H1 Hderiv2].
         apply determinist_exp_eval in H0 ; [|assumption]. apply H0 in H1. subst. f_equal. clear H0.
@@ -267,7 +270,7 @@ Qed.
 
 Definition _determinist_stmt_eval {S T : Set} (ext_exp_sem : @exp_sem_sig T) (stmt_sem : @stmt_sem_sig S T) : Prop := 
     @_determinist_exp_eval T ext_exp_sem  -> 
-    forall funs procs s env mem env' mem',  stmt_sem funs procs env mem s env' mem' ->  (forall env'' mem'', stmt_sem funs procs env mem s env'' mem'' -> env' = env'' /\ mem' = mem'').
+    forall funs procs s ev ev',  stmt_sem funs procs ev s ev' ->  (forall ev'', stmt_sem funs procs ev s ev'' -> ev' = ev'').
 
 
 Fact determinist_stmt_eval {S T : Set}: 
@@ -275,22 +278,22 @@ Fact determinist_stmt_eval {S T : Set}:
     @_determinist_stmt_eval S T ext_exp_sem ext_stmt_sem -> 
     _determinist_stmt_eval ext_exp_sem (@generic_stmt_sem S T ext_exp_sem ext_stmt_sem).
 Proof with auto. 
-    intros ext_exp_sem ext_stmt_sem Hds Hde funs procs s env mem env' mem' Hderiv. induction Hderiv ; intros.
+    intros ext_exp_sem ext_stmt_sem Hds Hde funs procs s ev ev' Hderiv. induction Hderiv ; intros.
     - inversion H... 
-    - inversion H3 ; subst ; split... repeat f_equal. apply determinist_exp_eval in H2...
-    - inversion H1 ; subst...  apply determinist_exp_eval in H7... destruct H. apply H7 in H. now symmetry in H.
-    - inversion H1 ; subst... apply determinist_exp_eval in H... destruct H7. apply H in H2. now symmetry in H2. 
+    - inversion H3 ; subst... repeat f_equal.  apply determinist_exp_eval in H2... apply H2 in H10. now subst.
+    - inversion H1 ; subst...  apply determinist_exp_eval in H6... destruct H. apply H6 in H. now symmetry in H.
+    - inversion H1 ; subst... apply determinist_exp_eval in H... destruct H6. apply H in H2. now symmetry in H2. 
     - inversion H0... 
-    - inversion H1 ; subst... apply IHHderiv in H4 as [Eq1 Eq2]. subst. apply IHHderiv0 in H7. now subst. 
+    - inversion H1 ; subst... apply IHHderiv in H4. subst. apply IHHderiv0 in H6. now subst. 
     - inversion H5 ; subst. 
        (* same args, same body *) 
             rewrite H10 in H0. injection H0 as H0. subst.
             (* same args eval *) 
-            assert (zargs = zargs0) by auto using (@Forall2_same_zargs T env mem eargs zargs zargs0 ext_exp_sem). 
-            subst. apply IHHderiv in H12 as [Eq1 Eq2]. subst. rewrite H4 in H16. injection H16 as H16. now subst.
-    - inversion H3.  subst. split... rewrite H7 in H0. injection H0 as Eq1. subst. 
-            assert (zargs = zargs0) by auto using (@Forall2_same_zargs T env'' mem eargs zargs zargs0 ext_exp_sem). subst. 
-            now apply IHHderiv in H11.
+            assert (zargs = zargs0) by auto using (@Forall2_same_zargs T ev eargs zargs zargs0 ext_exp_sem). 
+            subst. apply IHHderiv in H12. subst. rewrite H4 in H15. injection H15 as H15. now subst.
+    - inversion H3.  subst.  rewrite H7 in H0. injection H0 as Eq1. subst. 
+            assert (zargs = zargs0) by eauto using (@Forall2_same_zargs T _ eargs zargs zargs0 ext_exp_sem). subst. 
+            apply IHHderiv in H10. now subst.
     - inversion H0 ; subst... apply determinist_exp_eval in H... apply H in H2. injection H2 as H2. now subst.
     - inversion H1...
     - inversion H0. subst. unfold _determinist_stmt_eval in Hds. eapply Hds... apply H. apply H2.
@@ -302,8 +305,8 @@ Definition determinist_c_stmt_eval := determinist_stmt_eval Empty_exp_sem Empty_
 
 
 Definition _weakening_of_expression_semantics {T : Set} (exp_sem : @exp_sem_sig T) : Prop := 
-    forall e env mem (x:𝕍), 
-    exp_sem env mem e x <-> (forall env' mem',  (env,mem) ⊑ (env',mem') -> exp_sem env' mem' e x).
+    forall e ev (x:𝕍), 
+    exp_sem ev e x <-> (forall ev',  (ev ⊑ ev')%envmem -> exp_sem ev' e x).
 
 
 Lemma weakening_of_expression_semantics {T : Set} : 
@@ -317,21 +320,19 @@ Proof with (eauto using refl_env_mem_partial_order with rac_hint).
     - intro Hderiv. induction Hderiv; intros...
         + constructor. eapply eq_env_partial_order... easy.
         + unfold _weakening_of_expression_semantics in H. eapply  H in H2...
-            constructor... inversion H3. apply eq_env_partial_order with env... 
+            constructor... inversion H3. apply eq_env_partial_order with ev... 
 Qed.
 
 Fact _weakening_of_c_expression_semantics : _weakening_of_expression_semantics Empty_exp_sem. 
 Proof.
     unfold _weakening_of_expression_semantics. intros. split ; unfold Empty_exp_sem.
     - intros [].
-    - intro H. apply H with env mem... apply refl_env_mem_partial_order.
+    - intro H. apply H with ev... apply refl_env_mem_partial_order.
 Qed.
 
 Definition weakening_of_c_expression_semantics := 
     weakening_of_expression_semantics Empty_exp_sem _weakening_of_c_expression_semantics.
-Close Scope generic_sem_scope.
 
-Open Scope gmp_sem_scope.
 Lemma _weakening_of_gmp_expression_semantics : 
     _weakening_of_expression_semantics _gmp_exp_sem
 .
@@ -340,32 +341,27 @@ Proof with (eauto with rac_hint; try easy).
     - intro H. inversion H. subst. intros. apply GMP_E_Var with z; destruct H2 as [relEnv memEnv]. 
         + eapply eq_env_partial_order...
         + eapply eq_mem_partial_order... 
-    - intros. specialize H with env mem. now apply H.
+    - intros. specialize H with ev. now apply H.
 Qed.
-
 
 Definition weakening_of_gmp_expression_semantics := 
     weakening_of_expression_semantics _gmp_exp_sem _weakening_of_gmp_expression_semantics.
-Close Scope gmp_sem_scope.
-
-
-Open Scope generic_sem_scope.
 
 Definition _untouched_var_same_eval_exp {T : Set} (exp_sem : @exp_sem_sig T) := 
-    forall env mem (e: @_c_exp T) v x,
+    forall (ev:Env) (e: @_c_exp T) v x,
     ~ List.In v (exp_vars e) -> 
-    exp_sem env mem e x ->
-    (forall x', exp_sem((fst env){v\x'},snd env) mem e x)
+    exp_sem ev e x ->
+    (forall x', exp_sem (ev <| env ; vars ::= {{v\x'}} |>)  e x)
     /\ 
     (forall l z', 
-    _no_env_mpz_aliasing env ->
-    (fst env) v = Some (Def (VMpz (Some l))) -> exp_sem env mem{l\z'} e x).
+    _no_env_mpz_aliasing ev ->
+    ev v = Some (Def (VMpz (Some l))) -> exp_sem (ev <| mstate ::= {{l\z'}} |>) e x).
 
 Fact untouched_var_same_eval_exp {T : Set} : forall exp_sem, 
     _untouched_var_same_eval_exp exp_sem ->
     _untouched_var_same_eval_exp (@generic_exp_sem T exp_sem).
 Proof with eauto with rac_hint.
-    intros exp_sem Hext env mem e v x Hnotin Hderiv. induction Hderiv ; simpl in Hnotin...
+    intros exp_sem Hext ev e v x Hnotin Hderiv. induction Hderiv ; simpl in Hnotin...
     - split... constructor. simpl. apply p_map_not_same_eq...
     - rewrite List.in_app_iff in Hnotin ; apply Decidable.not_or_iff in Hnotin as [Hxnotine Hxnotine'].  split ; 
         intro x';  econstructor...
@@ -392,7 +388,7 @@ Qed.
 
 Fact _untouched_var_same_eval_exp_gmp : @_untouched_var_same_eval_exp _gmp_t _gmp_exp_sem.
 Proof.
-    intros env mem e v x Hnotin Hderiv. inversion Hderiv. subst. simpl in Hnotin.
+    intros ev e v x Hnotin Hderiv. inversion Hderiv. subst. simpl in Hnotin.
     apply Decidable.not_or_iff in Hnotin as [Hdiff _]. split...
     - econstructor. 
         * now apply p_map_not_same_eq.
@@ -408,23 +404,20 @@ Definition untouched_var_same_eval_exp_gmp := untouched_var_same_eval_exp _gmp_e
 
 
 Definition _untouched_var_same_eval_stmt {S T : Set} (exp_sem : @exp_sem_sig T) (stmt_sem : @stmt_sem_sig S T) := 
-    forall funs procs env mem env' mem' (s: @_c_statement S T) x, 
-    stmt_sem funs procs env mem s env' mem' ->
+    forall funs procs ev ev' (s: @_c_statement S T) x, 
+    stmt_sem funs procs ev s ev' ->
     ~ List.In x (stmt_vars s) /\ is_comp_var x = false -> 
-    (fst env) x = (fst env') x
+    ev x = ev' x
     .
 
 
-
-
-    
 Fact untouched_var_same_eval_stmt {S T : Set} : 
     forall exp_sem stmt_sem, 
     _untouched_var_same_eval_stmt exp_sem stmt_sem ->
     _untouched_var_same_eval_stmt exp_sem (@generic_stmt_sem S T exp_sem stmt_sem).
 Proof.
-    intros exp_sem stmt_sem Hext funs procs env mem env' mem' s x Hderiv [Hnotin Huservar]. induction Hderiv ; simpl in Hnotin; trivial.
-    - subst. apply Decidable.not_or_iff in Hnotin as [Hdiffxresf]. simpl. rewrite p_map_not_same.
+    intros exp_sem stmt_sem Hext funs procs ev ev' s x Hderiv [Hnotin Huservar]. induction Hderiv ; simpl in Hnotin; trivial.
+    - subst. apply Decidable.not_or_iff in Hnotin as [Hdiffxresf]. simpl. autounfold with rac_hint. rewrite p_map_not_same.
         * easy.
         * congruence.
     -  apply IHHderiv. 
@@ -441,9 +434,10 @@ Proof.
         + intro Hcontra. apply Hnotin. apply  List.in_app_iff. now left.
         + apply IHHderiv0. intro Hcontra. apply Hnotin. apply List.in_app_iff. now right.
     - simpl. symmetry. apply p_map_not_same_eq ; auto.
+    (* return *)
     - simpl. destruct (eq_dec res_f x). subst. 
         * discriminate.
-        * symmetry. rewrite p_map_not_same_eq. auto. congruence.     
+        * autounfold with rac_hint. symmetry. rewrite p_map_not_same_eq. auto. congruence.  
     - eapply Hext in H ; eauto.
 Qed.
 
@@ -452,10 +446,10 @@ Qed.
 
 Definition _weakening_of_statement_semantics_1  {S T : Set} (exp_sem : @exp_sem_sig T) (stmt_sem : @stmt_sem_sig S T) := 
     _weakening_of_expression_semantics exp_sem ->
-    forall (funs : @𝓕 S T) (procs : @𝓟 S T) Ω₀ M₀ s Ω₁ M₁,
-    stmt_sem funs procs Ω₀ M₀ s Ω₁ M₁ <->
-    ( forall Ω₀' M₀', (Ω₀ , M₀) ⊑ (Ω₀', M₀') ->
-    exists Ω₁' M₁', (Ω₁ , M₁) ⊑ (Ω₁', M₁') /\ stmt_sem funs procs Ω₀' M₀' s Ω₁' M₁').
+    forall (funs : @𝓕 S T) (procs : @𝓟 S T) ev₀ s ev₁,
+    stmt_sem funs procs ev₀ s ev₁ <->
+    ( forall ev₀', (ev₀  ⊑ ev₀')%envmem ->
+    exists ev₁' , (ev₁  ⊑ ev₁')%envmem /\ stmt_sem funs procs ev₀' s ev₁').
     
 
 Lemma weakening_of_statement_semantics_1 {S T : Set} : 
@@ -464,71 +458,69 @@ Lemma weakening_of_statement_semantics_1 {S T : Set} :
     -> _weakening_of_statement_semantics_1 exp_sem (@generic_stmt_sem S T exp_sem stmt_sem)
 .
 Proof with eauto using refl_env_mem_partial_order,env_partial_order_add with rac_hint.
-    intros exp_sem stmt_sem Hext_stmt Hext_exp funs procs Ω₀ M₀ s Ω₁ M₁. 
+    intros exp_sem stmt_sem Hext_stmt Hext_exp funs procs ev₀ s ev₁. 
     pose proof (weakening_of_expression_semantics exp_sem Hext_exp) as exp_weak.
     split.
-    - intro Hderiv. induction Hderiv ; intros Ω₀' M₀' [Henv Hmem].
+    - intro Hderiv. induction Hderiv ; intros ev₀' [Henv Hmem].
         (* skip *)
-        * exists Ω₀',M₀'... 
+        * exists ev₀'... 
         
         (* assign *) 
-        * exists ((fst Ω₀') {x \ z}, (snd Ω₀')) , M₀'. split.
-            + split...
+        * exists (ev₀' <| env ; vars ::= {{x \ z}} |>). split. 
+            + split... simpl. apply env_partial_order_add... 
             + apply S_Assign...
-                *** now apply env_same_ty with env. 
-                *** rewrite (exp_weak e) in H2. specialize (H2 Ω₀' M₀'). apply H2...
+                *** now apply env_same_ty with ev. 
+                *** rewrite (exp_weak e) in H2. specialize (H2 ev₀'). apply H2...
 
 
         (* if true *)
-        * destruct H. destruct (IHHderiv Ω₀' M₀') as [env_s [mem_s [[Henv2 Hmem2] Hderiv2]]]... exists env_s, mem_s. intros . split...
+        * destruct H. destruct (IHHderiv ev₀') as [ev_s [[Henv2 Hmem2] Hderiv2]]... exists ev_s. intros . split...
             apply S_IfTrue with z. split...
             rewrite  (exp_weak e) in H... apply Hderiv2...
         (* if false *)
-        * destruct (IHHderiv Ω₀' M₀') as [env_s [mem_s [[Henv2 Hmem2] Hderiv2]]]... exists env_s, mem_s. split...
+        * destruct (IHHderiv ev₀') as [ev_s [[Henv2 Hmem2] Hderiv2]]... exists ev_s. split...
             apply S_IfFalse...
             rewrite  (exp_weak e) in H... 
 
 
          (* while *)
-        * destruct (IHHderiv Ω₀' M₀') as [env_s [mem_s [[Henv2 Hmem2] Hderiv2]]]... exists env_s, mem_s.
-            intros. split... 
+        * destruct (IHHderiv ev₀') as [ev_s [[Henv2 Hmem2] Hderiv2]]... 
 
 
         (* c seq *)
-        *   destruct IHHderiv with Ω₀' M₀' as [I1env [I1mem [I1Hrel I1Hderiv]]]...
-            destruct IHHderiv0 with I1env I1mem as [I2env [I2mem [I2Hrel I2Hderiv]]]... 
+        * destruct IHHderiv with ev₀' as [I1ev [I1Hrel I1Hderiv]]...
+            destruct IHHderiv0 with I1ev as [I2ev [I2Hrel I2Hderiv]]... 
 
         (* f call *)
-         * specialize IHHderiv with (p_map_addall (H:=eqdec_v) ⊥ xargs zargs, ⊥)  M₀'. destruct IHHderiv as [env_s [mem_s [Hrel Hderiv2]]].
+         * edestruct IHHderiv as [e_s [Hrel Hderiv2]].
             + now split.
-            + eexists ?[env],?[mem]. split.
-                ++ instantiate (env:=((fst Ω₀') {c \Def z}, snd Ω₀')). instantiate (mem:=mem_s). split... easy. 
+            + eexists (ev₀' <| env; vars ::= {{c \Def z}} |> <| mstate := ev' |>). split.
+                ++ split... apply env_partial_order_add... easy. 
                 ++ eapply S_FCall... 
-                    +++ epose proof (List.Forall2_impl (R1:=generic_exp_sem env mem) (generic_exp_sem Ω₀' M₀')) as Hforall. destruct Hforall with eargs zargs... intros.
-                    apply exp_weak with env mem...
-                    +++ inversion Hrel. eapply eq_env_partial_order...
-
+                    +++ epose proof (List.Forall2_impl (R1:=generic_exp_sem ev) (generic_exp_sem ev₀')) as Hforall. destruct Hforall with eargs zargs...
+                        intros...
+                    apply exp_weak with ev...
         (* p call *)
-        * specialize IHHderiv with (p_map_addall (H:=eqdec_v) ⊥ xargs zargs, ⊥)  M₀'. destruct IHHderiv as [env_s [mem_s [Hrel Hderiv2]]].
+        *  edestruct IHHderiv as [ev_s [Hrel Hderiv2]].
             + now split... 
-            + repeat eexists... 
-                ++ destruct Hrel...
+            + eexists (_ <| mstate := _ |>)... simpl. split.
+                ++ destruct Hrel. split...
                 ++ eapply S_PCall ...
-                +++ epose proof (List.Forall2_impl (R1:=generic_exp_sem env mem) (generic_exp_sem Ω₀' M₀')) as Hforall. destruct Hforall with eargs zargs... intros.
-                    apply exp_weak with env mem...
+                    +++ epose proof (List.Forall2_impl (R1:=generic_exp_sem ev) (generic_exp_sem ev₀')) as Hforall. destruct Hforall with eargs zargs...
+                        intros. apply exp_weak with ev...
 
         (* return *)
-        * exists ((fst Ω₀') {res_f \Def z}, snd Ω₀'), M₀'. split.
-            + split...
-            + apply S_Return... apply (exp_weak e env mem z)...
+        * exists (ev₀' <| env ; vars ::= {{res_f \Def z}} |>). split.
+            + split... apply env_partial_order_add...
+            + apply S_Return... apply (exp_weak e ev z)...
 
         (* assert *)
-        * exists Ω₀', M₀'. split... apply S_PAssert with z...
-            apply (exp_weak e env mem z)...
+        * exists ev₀'. split... apply S_PAssert with z...
+            apply (exp_weak e ev z)...
 
         (* other cases *)
-        * specialize (Hext_stmt Hext_exp funs procs env mem (S_Ext s) env' mem').
-            apply Hext_stmt with Ω₀' M₀' in H. destruct H as [env'' [mem'' [Hrel2 Hderiv]]]... easy.
+        * specialize (Hext_stmt Hext_exp funs procs ev (S_Ext s) ev').
+            apply Hext_stmt with ev₀' in H. destruct H as [ev'' [Hrel2 Hderiv]]... easy.
                 
     - intros H. admit. (* ??? *)
         
@@ -539,9 +531,9 @@ Fact _weakening_of_c_statements_semantics_1 : _weakening_of_statement_semantics_
 Proof.
     unfold _weakening_of_statement_semantics_1. intros. split; unfold Empty_stmt_sem.
     - intros [].
-    - intro H2. destruct H2 with Ω₀ M₀.
+    - intro H2. destruct H2 with ev₀.
         + apply refl_env_mem_partial_order.
-        + destruct H0 as [_ [_ []]]. 
+        + destruct H0 as [_  []]. 
 Qed.
 
 
@@ -549,12 +541,12 @@ Lemma _weakening_of_gmp_statements_semantics_1 :
     _weakening_of_statement_semantics_1 _gmp_exp_sem _gmp_stmt_sem
 .
 Proof with eauto using eq_env_partial_order, eq_mem_partial_order,refl_env_mem_partial_order with rac_hint ; try easy.
-    intros Hweak funs procs Ω₀ M₀ s Ω₁ M₁. split.
-    - intro Hderiv. induction Hderiv; intros Ω₀' M₀' [Henv Hmem] ;
-        pose proof (fun y => weakening_of_gmp_expression_semantics y Ω₀ M₀) as weak_exp. 
+    intros Hweak funs procs ev₀ s ev₁. split.
+    - intro Hderiv. induction Hderiv; intros ev₀' [Henv Hmem] ;
+        pose proof (fun y => weakening_of_gmp_expression_semantics y ev₀) as weak_exp. 
 
         (* init *)
-        * exists ( (fst Ω₀') {x \ Def (VMpz (Some l))}, snd Ω₀'),  M₀'{l \Defined 0}. split.
+        * exists (ev₀' <| env ; vars ::= {{x \ Def (VMpz (Some l))}} |> <| mstate ::= {{l \Defined 0}} |> ). split.
             + split. 
                 ++ apply env_partial_order_add... 
                 ++ apply mems_partial_order_add...
@@ -570,44 +562,44 @@ Proof with eauto using eq_env_partial_order, eq_mem_partial_order,refl_env_mem_p
                     *)
                     admit.
         (* clear *)
-        * exists (p_map (fst Ω₀') (x, Def (VMpz None)), snd Ω₀'). eexists M₀' {a \ Undefined u}. split.
+        * exists (ev₀' <| env ; vars ::= {{x\Def (VMpz None)}} |><| mstate ::= {{a \ Undefined u}} |>). split.
             + split.
                 ++ apply env_partial_order_add...
                 ++ apply mems_partial_order_add...
             + constructor... 
 
-        * exists Ω₀',(M₀') {a \ Defined (z) ̇}. split.
-            + split... intro n. apply (mems_partial_order_add M₀ M₀' Hmem a (Int.to_z z)). 
+        * exists (ev₀' <| mstate ::= {{a \ Defined (z) ̇}} |>). split.
+            + split... intro n. apply (mems_partial_order_add ev₀ ev₀' Hmem a z ̇). 
             + apply S_set_i. eapply eq_env_partial_order... apply weak_exp...
 
-        * exists Ω₀', M₀' {a \ z}. split.
-            + split... intro n0.  apply (mems_partial_order_add M₀ M₀' Hmem a). 
+        * exists (ev₀' <| mstate ::= {{a \ z}} |>). split.
+            + split... intro n0.  apply (mems_partial_order_add ev₀ ev₀' Hmem a). 
             + apply S_set_z with n.
                 ++ eapply eq_env_partial_order...
                 ++ eapply eq_env_partial_order...
-                ++ apply (eq_mem_partial_order M₀ M₀')...
+                ++ apply (eq_mem_partial_order ev₀ ev₀')...
 
-        * inversion H0. subst. eexists (((fst Ω₀') {x \ Def (VInt (Int.mkMI z  ir))}, snd Ω₀')), M₀'... split.
-            + split... pose env_partial_order_add...
+        * inversion H0. subst. eexists (ev₀' <| env ; vars ::= fun e =>  e{x \ Def (VInt (z ⁱⁿᵗ ir))} |>)... split.
+            + split... simpl. pose proof env_partial_order_add...
             + apply S_get_int with v... apply weak_exp...
         
-        * exists Ω₀',M₀' {a \ Defined z}. split. 
-            + split... apply (mems_partial_order_add M₀ M₀' Hmem a z). 
+        * exists (ev₀' <| mstate ::= {{a \ Defined z}} |>). split. 
+            + split... apply (mems_partial_order_add ev₀ ev₀' Hmem a z). 
             + constructor...
 
         * inversion H. subst. inversion H8. inversion H0. subst. 
-            eexists ((fst Ω₀') {c \ b}, snd Ω₀'),M₀'. split.
-            ** split... pose env_partial_order_add...
+            eexists (ev₀' <| env ; vars ::= fun e => e{c \ b} |>). split.
+            ** split... simpl. pose env_partial_order_add...
             ** inversion H13. subst. apply S_cmp with vx vy lx ly...
                 + constructor... 
                 + constructor...
         
-        * eexists Ω₀', M₀' {lr \Defined (⋄ (□ bop) z1 z2)}. split.
+        * eexists (ev₀' <| mstate ::= {{lr \Defined (⋄ bop z1 z2)}} |>). split.
             ** split... intro n. apply mems_partial_order_add...
             **  apply S_op with vx vy ; try apply weak_exp...
     
-    - intro H. specialize (H Ω₀ M₀ (refl_env_mem_partial_order Ω₀ M₀))...
-        destruct H as [Ω₁' [M₁' [Hrel Hderiv ]]]... induction Hderiv.
+    - intro H. specialize (H ev₀ (refl_env_mem_partial_order ev₀))...
+        destruct H as [ev₁' [Hrel Hderiv ]]... induction Hderiv.
         + admit. (* non sense ? *)
 Admitted.
 
@@ -619,17 +611,17 @@ Definition weakening_of_gmp_statements_semantics_1 :=
 
 Definition _weakening_of_statement_semantics_2  {S T : Set} (exp_sem : @exp_sem_sig T) (stmt_sem : @stmt_sem_sig S T) := 
     
-    forall (funs : @𝓕 S T) (procs : @𝓟 S T) Ω₀ Ω₀' M₀ M₀' s Ω₁ M₁,
+    forall (funs : @𝓕 S T) (procs : @𝓟 S T) ev₀ ev₀' s ev₁,
     _determinist_exp_eval exp_sem ->
     _weakening_of_expression_semantics exp_sem ->
-    stmt_sem funs procs Ω₀ M₀ s Ω₁ M₁ /\ (Ω₀, M₀) ⊑ (Ω₀', M₀')  ->
+    stmt_sem funs procs ev₀ s ev₁ /\ (ev₀ ⊑ ev₀')%envmem  ->
     (
-        forall Ω₁' M₁',
-        stmt_sem funs procs Ω₀' M₀' s Ω₁' M₁'->
+        forall ev₁',
+        stmt_sem funs procs ev₀' s ev₁'->
         (* if v is a compiler variable, i.e. a function return value, v can change*)
-        (forall (v:𝓥), (v ∉ fst Ω₀) /\ is_comp_var v = false  -> fst Ω₀' v = fst Ω₁' v) 
+        (forall (v:𝓥), (v ∉ ev₀) /\ is_comp_var v = false  -> ev₀' v = ev₁' v) 
         /\
-        (forall (x:location) (v:𝓥), (fst Ω₀ v) <> Some (Def (VMpz x)) -> M₀' x = M₁' x)
+        (forall (x:location) (v:𝓥), ev₀ v <> Some (Def (VMpz x)) -> ev₀'.(mstate) x = ev₁'.(mstate) x)
     ).
 
 
@@ -639,23 +631,23 @@ Lemma weakening_of_statement_semantics_2 {S T : Set} :
     -> _weakening_of_statement_semantics_2 exp_sem (@generic_stmt_sem S T exp_sem stmt_sem)
 .
 Proof with auto with rac_hint.
-    intros exp_sem stmt_sem ext_stmt_weak funs procs Ω₀ Ω₀' M₀ M₀' s Ω₁ M₁ ext_exp_deter ext_exp_weak  [Hderiv1 Hrel].
+    intros exp_sem stmt_sem ext_stmt_weak funs procs ev₀ ev₀' s ev₁ ext_exp_deter ext_exp_weak  [Hderiv1 Hrel].
     pose proof (weakening_of_expression_semantics exp_sem ext_exp_weak) as exp_weak.
     unfold _weakening_of_expression_semantics in exp_weak.
     unfold _weakening_of_statement_semantics_2 in ext_stmt_weak.
     
-    induction Hderiv1 ; intros Ω₁' M₁' Hderiv2 ; inversion Hderiv2 ; subst ; try easy...
+    induction Hderiv1 ; intros ev₁' Hderiv2 ; inversion Hderiv2 ; subst ; try easy...
     
     (* assign *)
-    - split... simpl. intros v [Hnotin Hnotcompvar].  assert (HH: type_of_value (fst env x) <> None) by congruence. apply type_of_value_env in HH.
-        apply not_in_diff with (x:=v)  in HH... eapply p_map_not_same_eq... intro neq...
+    - split... simpl. intros v [Hnotin Hnotcompvar].  assert (HH: type_of_value (ev x) <> None) by congruence. apply type_of_value_env in HH.
+        apply not_in_diff with (x:=v)  in HH... autounfold with rac_hint. eapply p_map_not_same_eq...  intro neq...
 
     (* if false *)
-    - apply IHHderiv1... destruct H. specialize (exp_weak e env mem z). rewrite exp_weak in H. specialize (H Ω₀' M₀' Hrel). 
-            apply determinist_exp_eval in H. apply H in H6. now subst. assumption.
+    - apply IHHderiv1... destruct H. specialize (exp_weak e ev z). rewrite exp_weak in H. specialize (H ev₀' Hrel). 
+            apply determinist_exp_eval in H. apply H in H5. now subst. assumption.
 
     (* if true *)
-    -  destruct H6. specialize (exp_weak e env mem zero). rewrite exp_weak in H. specialize (H Ω₀' M₀' Hrel).
+    -  destruct H5. specialize (exp_weak e ev (VInt zero)). rewrite exp_weak in H. specialize (H ev₀' Hrel).
             apply determinist_exp_eval in H. apply H in H1. now subst. assumption.
 
     (* seq *)
@@ -666,7 +658,7 @@ Proof with auto with rac_hint.
 
     (* pcall *)
     - rewrite H6 in H0. injection H0 as H0. subst. edestruct IHHderiv1... admit. admit.
-        epose proof (List.Forall2_impl (R1:=generic_exp_sem env mem) (generic_exp_sem env mem)) as Hforall. admit.
+        epose proof (List.Forall2_impl (R1:=generic_exp_sem ev) (generic_exp_sem ev)) as Hforall. admit.
 
     (* return *)
     -  split ; intros v... intros [Hnotin Hnotcomp]. destruct (string_dec res_f v).
@@ -674,23 +666,23 @@ Proof with auto with rac_hint.
         +  symmetry. apply p_map_not_same...
             
     (* assert *)
-    - eapply ext_stmt_weak with ( Ω₀:=env) ( M₀:=mem) (Ω₁:=env') (M₁:=mem') in H1...
+    - eapply ext_stmt_weak with (ev₀:=ev) (ev₁:=ev')  in H1...
 Admitted.
 
 
 (* 3 *)
 
 Definition _weakening_of_expression_semantics_3 {T : Set} (exp_sem : @exp_sem_sig T) := 
-    forall env mem e z Ω₀ M₀,
-    exp_sem env mem e z ->
-    forall Ω₀' M₀', (Ω₀', M₀') ⊑ (Ω₀, M₀) ->
+    forall ev e z ev₀,
+    exp_sem ev e z ->
+    forall ev₀', (ev₀' ⊑ ev₀)%envmem ->
     (
-        (forall v, (dom (fst Ω₀) - dom (fst Ω₀')) v /\ ~ List.In v (exp_vars e))
+        (forall v, (dom ev₀ - dom ev₀') v /\ ~ List.In v (exp_vars e))
         /\
-        (forall x v, (dom M₀ - dom M₀') x -> (fst Ω₀) v = Some (Def (VMpz x)) /\ ~ List.In v (exp_vars e))
+        (forall x v, (dom ev₀.(mstate) - dom ev₀'.(mstate)) x ->  ev₀ v = Some (Def (VMpz x)) /\ ~ List.In v (exp_vars e))
     ) ->
 
-    exp_sem  Ω₀' M₀' e z
+    exp_sem  ev₀' e z
 .
 
 Fact weakening_of_expression_semantics_3 {S T : Set} : forall exp_sem, 
@@ -698,7 +690,7 @@ Fact weakening_of_expression_semantics_3 {S T : Set} : forall exp_sem,
     -> _weakening_of_expression_semantics_3 (@generic_exp_sem T exp_sem)
 .
 Proof with auto.
-    intros exp Hweak env mem e v env1 mem1 Hderiv env2 mem2 Hrel [Henv Hmem]. induction Hderiv.
+    intros exp Hweak ev e v ev1 Hderiv ev2 Hrel [Henv Hmem]. induction Hderiv.
     - constructor.
     - constructor. destruct Henv with x. simpl in H1. destruct H1. now left.
     - econstructor.
@@ -741,17 +733,17 @@ Proof with auto.
 Qed.
 
 Definition _weakening_of_statement_semantics_3  {S T : Set} (stmt_sem : @stmt_sem_sig S T) := 
-    forall funs procs Ω₀ M₀  s Ω₁ M₁,
-    stmt_sem funs procs Ω₀ M₀ s Ω₁ M₁ -> 
+    forall funs procs ev₀  s ev₁,
+    stmt_sem funs procs ev₀ s ev₁ -> 
     (
-        forall Ω₀' M₀', (Ω₀', M₀') ⊑ (Ω₀, M₀) ->
+        forall ev₀', (ev₀' ⊑ ev₀)%envmem ->
         (
-            (forall v, (dom (fst Ω₀) - dom (fst Ω₀')) v /\ ~ List.In v (stmt_vars s))
+            (forall v, (dom ev₀ - dom ev₀') v /\ ~ List.In v (stmt_vars s))
             /\
-            (forall x v, (dom M₀ - dom M₀') x -> (fst Ω₀) v = Some (Def (VMpz x)) /\ ~ List.In v (stmt_vars s))
+            (forall x v, (dom ev₀.(mstate) - dom ev₀'.(mstate)) x -> ev₀ v = Some (Def (VMpz x)) /\ ~ List.In v (stmt_vars s))
         ) ->
 
-        exists Ω₁' M₁', stmt_sem funs procs Ω₀' M₀' s Ω₁' M₁'
+        exists ev₁', stmt_sem funs procs ev₀' s ev₁'
     ).
 
 Lemma weakening_of_statement_semantics_3 {S T : Set} : 
@@ -762,20 +754,20 @@ Lemma weakening_of_statement_semantics_3 {S T : Set} :
 .
 
 Proof with auto with rac_hint.
-    intros exp_sem stmt_sem ext_exp_weak ext_stmt_weak funs procs Ω₀ M₀ s Ω₁ M₁ Hderiv Ω₀' M₀' Hrel [Henv Hmem].
+    intros exp_sem stmt_sem ext_exp_weak ext_stmt_weak funs procs ev₀ s ev₁ Hderiv ev₀' Hrel [Henv Hmem].
     induction Hderiv.
     (* skip *)
-    - exists Ω₀', M₀'. constructor.
+    - exists ev₀'. constructor.
     (* assign *)
     - destruct Henv with x. simpl in H4. destruct H4...  
     (* if true *)
-    - destruct IHHderiv as [env'' [mem'' Hx]]...
+    - destruct IHHderiv as [ev'' Hx]...
         + intro v. destruct Henv with v. split... intros Hin. apply H2.
             apply List.in_app_iff. right. apply List.in_app_iff...
         + intros l v Hdom. destruct Hmem with l v... split... intros Hin. apply H2.  
             apply List.in_app_iff. right. apply List.in_app_iff...
-        + exists env'', mem''. apply S_IfTrue with z... destruct H as [He Hzero]. split...
-            eapply weakening_of_expression_semantics_3 in He... specialize He with Ω₀' M₀'. apply He.
+        + exists ev''. apply S_IfTrue with z... destruct H as [He Hzero]. split...
+            eapply weakening_of_expression_semantics_3 in He... specialize He with ev₀'. apply He.
             * apply Hrel.
             * split ; simpl in Henv,Hmem.
                 ** intros v. specialize Henv with v as [He1 He2]. simpl in He2. split...
@@ -784,13 +776,13 @@ Proof with auto with rac_hint.
                     intro Hin. apply Hm2. apply List.in_app_iff...
 
     (* if false *)
-    - destruct IHHderiv as [env'' [mem'' Hx]]...
+    - destruct IHHderiv as [ev'' Hx]...
         + intro v. destruct Henv with v. split... intros Hin. apply H2.
             apply List.in_app_iff. right. apply List.in_app_iff...
         + intros l v Hdom. destruct Hmem with l v... split... intros Hin. apply H2.  
             apply List.in_app_iff. right. apply List.in_app_iff...
-        + exists env'', mem''. apply S_IfFalse... 
-            eapply weakening_of_expression_semantics_3 in H... specialize H with Ω₀' M₀'. apply H.
+        + exists ev''. apply S_IfFalse... 
+            eapply weakening_of_expression_semantics_3 in H... specialize H with ev₀'. apply H.
             * apply Hrel.
             * split ; simpl in Henv,Hmem.
                 ** intros v. specialize Henv with v as [He1 He2]. simpl in He2. split...
@@ -798,7 +790,7 @@ Proof with auto with rac_hint.
                 ** intros x v Hdom. specialize Hmem with x v. apply Hmem in Hdom as [Hm1 Hm2]. simpl in Hm2. split...
                     intro Hin. apply Hm2. apply List.in_app_iff...
     (* while *)
-    - destruct IHHderiv as [env'' [mem'' Hx]]...
+    - destruct IHHderiv as [ev'' Hx]...
         + intro v. destruct Henv with v. split... intros Hin. simpl in H1,Hin. apply H1. rewrite List.app_nil_r in Hin.
             apply List.in_app_iff in Hin. destruct Hin.
             * apply List.in_app_iff...
@@ -807,43 +799,40 @@ Proof with auto with rac_hint.
             apply List.in_app_iff in Hin. destruct Hin.
             * apply List.in_app_iff...
             * apply List.in_app_iff in H2. destruct H2... apply List.in_app_iff...
-        +  exists env'', mem''. constructor... 
+        +  exists ev''. constructor... 
 
     (* seq *)
-    - destruct IHHderiv as [env0 [mem0 Hx]]...
+    - destruct IHHderiv as [ev0 Hx]...
         + intro v. destruct Henv with v. split... intros Hin. simpl in H2,Hin. apply H2. 
             apply List.in_app_iff...
         + intros l v Hdom. destruct Hmem with l v... split... intros Hin. apply H2. simpl in Hin.
             apply List.in_app_iff...
-        + eexists. eexists. apply S_Seq with env0 mem0... admit. 
+        + eexists.  apply S_Seq with ev0... admit. 
 
     (* fcall *)
-    - eexists. eexists. apply S_FCall with b env' xargs zargs...
+    - eexists. apply S_FCall with b xargs zargs...
         * admit.
         * admit.
         * apply H4.
 
     (* pcall *)
-    - repeat eexists. apply S_PCall with b env' xargs zargs...
+    - repeat eexists. apply S_PCall with b xargs zargs...
         * admit.
         *  admit.
 
     (* return *)
-    - exists ((fst Ω₀'){res_f\Def z},snd Ω₀').  eexists M₀'. apply S_Return.
-        eapply weakening_of_expression_semantics_3 in H... specialize H with Ω₀' M₀'. apply H...
-        * apply Hrel.
-        * easy. 
+    - exists (ev₀' <| env ; vars ::= {{res_f\Def z}} |>). apply S_Return.
+        eapply weakening_of_expression_semantics_3 in H... specialize H with ev₀'. apply H... apply Hrel.
         
     (* assert *)
-    - exists Ω₀'. exists M₀'. apply S_PAssert with z... 
-        eapply weakening_of_expression_semantics_3 in H... specialize H with Ω₀' M₀'. apply H...
-        * apply Hrel.
-        * easy.
+    - exists ev₀'. apply S_PAssert with z... 
+        eapply weakening_of_expression_semantics_3 in H... specialize H with ev₀'. apply H... apply Hrel.
+        
 
     (* other cases *)
     - unfold _weakening_of_statement_semantics_3 in ext_stmt_weak.
-        specialize (ext_stmt_weak funs procs  env mem (S_Ext s) _ _ H Ω₀' M₀' Hrel).
-        destruct ext_stmt_weak as [env'' [mem'' Hd]]... exists env'', mem''...
+        specialize (ext_stmt_weak funs procs  ev (S_Ext s) _ H ev₀' Hrel).
+        destruct ext_stmt_weak as [ev'' Hd]... exists ev''...
 Admitted.
 
 
@@ -880,12 +869,12 @@ Qed.
 
 Open Scope macro_sem_scope.
 
-Corollary same_eval_macro :  forall Ω M v l e z z', 
-    _no_env_mpz_aliasing Ω ->
+Corollary same_eval_macro :  forall (ev : Env) v l e z z', 
+    _no_env_mpz_aliasing ev ->
     ~ List.In v (exp_vars e) ->
-    (fst Ω) v = Some (Def (VMpz (Some l))) ->
-    Ω ⋅ M |= e ⇝ z ->
-    Ω ⋅ (M) {l \ Defined z'} |= e ⇝ z.
+    ev v = Some (Def (VMpz (Some l))) ->
+    ev |= e ⇝ z ->
+    ev <| mstate ::= {{l \ Defined z'}} |> |= e ⇝ z.
 
 Proof.
     intros. inversion H2.
@@ -899,10 +888,10 @@ Proof.
 Qed.
 
 Lemma semantics_of_the_mpz_assgn_macro :
-    forall funs procs e z Ω M v (y:location),
-    Ω ⋅ M |= e ⇝ z ->
-    (fst Ω) v = Some (Def (VMpz y)) ->
-    gmp_stmt_sem funs procs Ω M (mpz_ASSGN v e) Ω M{y\Defined z} 
+    forall funs procs e z (ev : Env) v (y:location),
+    ev |= e ⇝ z ->
+    ev v = Some (Def (VMpz y)) ->
+    gmp_stmt_sem funs procs ev (mpz_ASSGN v e) (ev <| mstate ::= {{y\Defined z}} |>)
 .
 Proof.
     intros. 
@@ -917,14 +906,14 @@ Proof.
 Qed.
 
 Lemma semantics_of_the_int_assgn_macro :
-    forall funs procs e z (ir: Int.inRange z) Ω M v,
+    forall funs procs e z (ir: Int.inRange z) (ev:Env) v,
     is_comp_var v = false ->
-    Ω ⋅ M |= e ⇝ z ->
-    type_of_value ((fst Ω) v) = Some C_Int ->
-    gmp_stmt_sem funs procs Ω M (int_ASSGN v e) ((fst Ω){v\z ⁱⁿᵗ ir : 𝕍}, snd Ω)  M
+    ev |= e ⇝ z ->
+    type_of_value (ev v) = Some C_Int ->
+    gmp_stmt_sem funs procs ev (int_ASSGN v e) (ev <| env ; vars ::= {{v\VInt (z ⁱⁿᵗ ir) : 𝕍}} |>)
 .
 Proof with eauto with rac_hint.
-    intros funs procs e z ir Ω M v Hnotcomp H H0. 
+    intros funs procs e z ir ev v Hnotcomp H H0. 
     unfold int_ASSGN.
     destruct (ty e)  eqn:EqTY.
     - constructor... inversion H ; subst.
@@ -936,19 +925,19 @@ Proof with eauto with rac_hint.
 Qed.
 
 Lemma semantics_of_the_Z_assgn_macro_tint :
-    forall funs procs z (ir: Int.inRange z) Ω M v,
+    forall funs procs z (ir: Int.inRange z) (ev:Env) v,
     is_comp_var v = false ->
-    type_of_value ((fst Ω) v) = Some C_Int ->
-    gmp_stmt_sem funs procs Ω M (Z_ASSGN C_Int v z) ((fst Ω){v\z ⁱⁿᵗ ir : 𝕍}, snd Ω) M
+    type_of_value (ev v) = Some C_Int ->
+    gmp_stmt_sem funs procs ev (Z_ASSGN C_Int v z) (ev <| env ; vars ::= {{v\VInt (z ⁱⁿᵗ ir) : 𝕍}} |>)
 .
 Proof.
     intros.  constructor ; auto with rac_hint.
 Qed.
 
 Lemma semantics_of_the_Z_assgn_macro_tmpz :
-    forall funs procs y (z:ℤ) Ω M v,
-    (fst Ω) v = Some (Def (VMpz (Some y))) ->
-    gmp_stmt_sem funs procs Ω M (Z_ASSGN Mpz v z) Ω M{y\Defined z}
+    forall funs procs y (z:ℤ) (ev:Env) v,
+    ev v = Some (Def (VMpz (Some y))) ->
+    gmp_stmt_sem funs procs ev (Z_ASSGN Mpz v z) (ev <| mstate ::= {{y\Defined z}} |>)
 .
 Proof with auto using BinaryString.Z_of_of_Z.
     intros. simpl. constructor. apply S_set_s...
@@ -956,12 +945,12 @@ Qed.
 
 
 Lemma semantics_of_the_cmp_macro :
-    forall funs procs (Ω:Ω) (M:𝓜) c e1 e2 v1 v2 z1 z2 a,
-    _no_env_mpz_aliasing Ω ->
+    forall funs procs (ev:Env) c e1 e2 v1 v2 z1 z2 a,
+    _no_env_mpz_aliasing ev ->
     is_comp_var c = false ->
-    type_of_value ((fst Ω) c) = Some C_Int ->
-    Ω ⋅ M |= e1 ⇝ z1 ->
-    Ω ⋅ M |= e2 ⇝ z2 ->
+    type_of_value (ev c) = Some C_Int ->
+    ev |= e1 ⇝ z1 ->
+    ev |= e2 ⇝ z2 ->
 
     (
         (Def a = VInt sub_one <-> Z.lt z1 z2 ) /\
@@ -971,43 +960,50 @@ Lemma semantics_of_the_cmp_macro :
 
     (* v1 and v2 must be bound to a mpz location (implied by mpz_assign ) *)
     forall (l1 l2 : location),
-    (fst Ω) v1 = Some (Def (VMpz l1)) /\  (fst Ω) v2 = Some (Def (VMpz l2))->
+    ev v1 = Some (Def (VMpz l1)) /\  ev v2 = Some (Def (VMpz l2))->
     
     ~ List.In v1 ((exp_vars e2)) /\  l1 <> l2   -> (* not in paper proof *)
 
-    exists M', (
+    exists M, (
         forall v (n:location), 
-        (fst Ω) v = Some (Def (VMpz n)) ->
-        (fst Ω) v <> (fst Ω) v1 /\ (fst Ω) v <> (fst Ω) v2  -> 
-        M n = M' n
+        ev v = Some (Def (VMpz n)) ->
+        ev v <> ev v1 /\ ev v <> ev v2  -> 
+        ev.(mstate) n = M n
     ) -> 
     
-    gmp_stmt_sem funs procs Ω M (CMP c e1 e2 v1 v2) ((fst Ω){c\Def a}, snd Ω) M'
+    gmp_stmt_sem funs procs ev (CMP c e1 e2 v1 v2) (ev <| env ; vars ::= {{c\Def a}} |> <| mstate := M |>) 
 .
 
 Proof with try easy ; auto with rac_hint ; unshelve eauto using Z.ltb_irrefl,Z.gtb_ltb,Z.ltb_lt with rac_hint; auto with rac_hint.
-    intros funs procs Ω M c e1 e2 v1 v2 z1 z2 a Hnoalias Hnocom H H0 H1 (inf & eq & sup) l1 l2 (Hv1 & Hv2) (Hv1NotIne2 & Hdiffl1l2).
+    intros funs procs ev c e1 e2 v1 v2 z1 z2 a Hnoalias Hnocom H H0 H1 (inf & eq & sup) l1 l2 (Hv1 & Hv2) (Hv1NotIne2 & Hdiffl1l2).
     
     assert (NotInt : 
-        exists M', (
+        exists M, (
             forall v (n:location), 
-            (fst Ω) v = Some (Def (VMpz n)) ->
-            (fst Ω) v <> (fst Ω) v1 /\ (fst Ω) v <> (fst Ω) v2  -> 
-                M n = M' n
+            ev v = Some (Def (VMpz n)) ->
+            ev v <> ev v1 /\ ev v <> ev v2  -> 
+            ev.(mstate) n = M n
         ) -> 
-        gmp_stmt_sem funs procs Ω M <{(mpz_ASSGN v1 e1); (mpz_ASSGN v2 e2); <c = cmp (v1, v2)>}> ((fst Ω) {c \Def a}, snd Ω)  M'
+        gmp_stmt_sem funs procs ev <{(mpz_ASSGN v1 e1); (mpz_ASSGN v2 e2); <(c = cmp (v1, v2) )>}> 
+        (ev <| env ; vars ::= {{c \Def a}} |> <| mstate := M |>)
     ). {
-        exists M{l2 \Defined z2, l1 \Defined  z1}. intros Hvdiff. apply S_Seq with Ω M{l1\Defined z1}.
+        exists ev.(mstate){l2 \Defined z2, l1 \Defined  z1}. intros Hvdiff. 
+        apply S_Seq with (ev <| mstate ::= {{l1\Defined z1}} |>).
         - apply semantics_of_the_mpz_assgn_macro...
-        - eapply S_Seq with Ω M{l2\Defined z2,l1\Defined z1}.
+        - eapply S_Seq with (ev <| mstate ::= {{l1\Defined z1}} |> <| mstate ::= {{l2\Defined z2}} |> ).
             + apply semantics_of_the_mpz_assgn_macro... inversion H1 ; subst. 
                 * constructor. eapply untouched_var_same_eval_exp_gmp...
-                * inversion H2. subst.   assert (Hdiffxv1: x <> v1). { simpl in Hv1NotIne2. now apply Decidable.not_or_iff in Hv1NotIne2 as [Hv1NotIne2 _]. }
-                    econstructor. eapply untouched_var_same_eval_exp_gmp... assert (Hdiffll1: l <> l1)... apply p_map_not_same_eq...
+                * inversion H2. subst.   assert (Hdiffxv1: x <> v1). 
+                    { simpl in Hv1NotIne2. now apply Decidable.not_or_iff in Hv1NotIne2 as [Hv1NotIne2 _]. }
+                    econstructor. eapply untouched_var_same_eval_exp_gmp... 
+                    assert (Hdiffll1: l <> l1)... apply p_map_not_same_eq... 
 
-            + constructor. apply S_cmp with (vx:=l1) (vy:=l2) (lx:=z1) (ly:=z2)...
+            + constructor. replace 
+                (_ <| env; vars ::= _ |><| mstate := _ |>)
+                with (ev <| mstate := ev.(mstate) {l2 \Defined z2, l1 \Defined z1} |><| env; vars ::= {{c \Def a}} |> ) by reflexivity.
+                apply S_cmp with (vx:=l1) (vy:=l2) (lx:=z1) (ly:=z2) ; simpl...
                 * constructor... constructor 1 with z1...  apply p_map_not_same_eq...
-                * constructor...
+                * constructor... constructor 1 with z2...  apply p_map_same...
                 * apply p_map_not_same_eq...
     }
     unfold CMP. destruct (ty e1) eqn:T1, (ty e2) eqn:T2 ; try apply NotInt ; clear NotInt.
@@ -1015,95 +1011,100 @@ Proof with try easy ; auto with rac_hint ; unshelve eauto using Z.ltb_irrefl,Z.g
     (* both ty(e1) = int and ty(e2) = int *)
     inversion H0 ; inversion H1 ; try 
     match goal with 
-    | Contra :  (_ ⋅ _ |= _ => Def (VMpz _))%gmpsem |- _ => 
+    | Contra :  (_ |= _ => Def (VMpz _))%gmpesem |- _ => 
         inversion Contra ; match goal with 
-        | Contra : _gmp_exp_sem _ _ _ _ |- _ => inversion Contra ; now subst
+        | Contra : _gmp_exp_sem _ _ _ |- _ => inversion Contra ; now subst
         end
     end.
 
-    exists M. intros Hvdiff. clear Hvdiff (* not needed *). destruct (Z.lt_trichotomy z1 z2) as [inf' | [ eq' | sup']].
+    exists ev.(mstate). intros Hvdiff. clear Hvdiff (* not needed *). destruct (Z.lt_trichotomy z1 z2) as [inf' | [ eq' | sup']].
         
     (* z1 < z2 *)
     * assert (cmp := inf'). apply <- inf in inf'. clear eq inf sup. subst.
-        destruct x,x0. subst. apply S_IfTrue with one.
-        + split... apply C_E_BinOpTrue with val val0 in_range in_range0... apply Z.ltb_lt. apply cmp.
-        + inversion inf'. constructor...  apply (C_E_BinOpInt Ω M 0 1 0 1) with zeroinRange oneinRange...
+        destruct x,x0. subst. apply S_IfTrue with (VInt one).
+        + split... apply C_E_BinOpTrue with x x0 i i0... apply Z.ltb_lt. apply cmp.
+        + inversion inf'. constructor...  apply (C_E_BinOpInt ev 0 1 0 1) with zeroinRange oneinRange...
 
     (* z1 = z2 *)
     * assert (cmp := eq'). rewrite <- eq in eq'. clear eq inf sup. subst.
-        destruct x,x0. apply Int.mi_eq in cmp. injection cmp as cmp. inversion eq'. subst. constructor...
+        destruct x,x0. apply Int.mi_eq in cmp. injection cmp as cmp. inversion eq'. subst. repeat constructor... 
 
     (* z1 > z2 *)
     * assert (cmp := sup').  apply Z.lt_gt in sup'. apply <- sup in sup'.  clear inf eq sup. subst.
         destruct x, x0. subst. constructor ; simpl in *.
         + eapply C_E_BinOpFalse... apply Z.ltb_ge. unfold Z.le. now rewrite cmp.  
-        + inversion sup'. subst. apply S_IfTrue with one.
-            ++  subst. split... apply C_E_BinOpTrue with val val0 in_range in_range0... now apply Z.gtb_lt.
-            ++  constructor... 
+        + inversion sup'. subst. apply S_IfTrue with (VInt one).
+            ++  subst. split... apply C_E_BinOpTrue with x x0 i i0... now apply Z.gtb_lt.
+            ++  constructor...
 Qed.
 
 
 
 
 Lemma semantics_of_the_binop_macro_int :
-    forall funs procs (Ω:Ω) (M:𝓜) (op:fsl_binop_int) c r e1 e2 v1 v2 z1 z2 (ir: Int.inRange (⋄ (□ op) z1 z2) ) l1 l2 lr,
-    _no_env_mpz_aliasing Ω ->
+    forall funs procs (ev:Env) (op:fsl_binop_int) c r e1 e2 v1 v2 z1 z2 (ir: Int.inRange (⋄ op z1 z2) ) l1 l2 lr,
+    _no_env_mpz_aliasing ev ->
     is_comp_var c = false ->
-    type_of_value ((fst Ω) c) = Some C_Int ->
-    Ω ⋅ M |= e1 ⇝ z1 ->
-    Ω ⋅ M |= e2 ⇝ z2 ->
-    let zr := ⋄ (□ op) z1 z2 in
+    type_of_value (ev c) = Some C_Int ->
+    ev |= e1 ⇝ z1 ->
+    ev |= e2 ⇝ z2 ->
+    let zr := ⋄ op z1 z2 in
 
-    (fst Ω) v1 = Some (Def (VMpz (Some l1))) /\  
-    (fst Ω) v2 = Some (Def (VMpz (Some l2))) /\
-    (fst Ω) r = Some (Def (VMpz (Some lr))) ->
-    exists M', (forall v n, (fst Ω) v = Some (Def (VMpz (Some n))) ->
-    ~ ((fst Ω) v1 = (fst Ω) v) /\ ~ ((fst Ω) v2 = (fst Ω) v)  -> M n = M' n) -> 
+    ev v1 = Some (Def (VMpz (Some l1))) /\  
+    ev v2 = Some (Def (VMpz (Some l2))) /\
+    ev r = Some (Def (VMpz (Some lr))) ->
+    exists M, (forall v n, ev v = Some (Def (VMpz (Some n))) ->
+    ev v1 <> ev v /\ ev v2 <> ev v  -> ev.(mstate) n = M n) -> 
 
     ~ List.In v1 ((exp_vars e2)) /\  l1 <> l2   -> (* not in paper proof *)
 
-    gmp_stmt_sem funs procs Ω M (binop_ASSGN op (C_Int,c) e1 e2 r v1 v2) ((fst Ω){c\zr ⁱⁿᵗ ir : 𝕍}, snd Ω) M'
+    gmp_stmt_sem funs procs ev (binop_ASSGN op (C_Int,c) e1 e2 r v1 v2) (ev <| env ; vars ::= fun e => e{c\VInt (zr ⁱⁿᵗ ir) : 𝕍} |> <| mstate := M |>)
     .
 
 Proof with eauto with rac_hint.
-    intros funs procs Ω M op c r e1 e2 v1 v2 z1 z2 ir l1 l2 lr Hnoalias Hnocomp H H0 H1 zr H2. destruct H2 as (v1l & v2l & rl).  
+    intros funs procs ev op c r e1 e2 v1 v2 z1 z2 ir l1 l2 lr Hnoalias Hnocomp H H0 H1 zr H2. destruct H2 as (v1l & v2l & rl).  
     assert (NotInt : 
-        exists M',
+        exists M,
         (forall (v : 𝓥) (n : location),
-        fst Ω v = Some (Def (VMpz n)) ->
-        fst Ω v1 <> fst Ω v /\ fst Ω v2 <> fst Ω v ->
-        M n = M' n) ->
+        ev v = Some (Def (VMpz n)) ->
+        ev v1 <> ev v /\ ev v2 <> ev v ->
+        ev.(mstate) n = M n) ->
         ~ List.In v1 ((exp_vars e2)) /\  l1 <> l2   -> (* not in paper proof *)
-        gmp_stmt_sem funs procs Ω M <{
+        gmp_stmt_sem funs procs ev <{
             (mpz_ASSGN v1 e1);
             (mpz_ASSGN v2 e2);
             (Definitions.op op r v1 v2);
             (int_ASSGN c (C_Id r Mpz))
-        }> ((fst Ω) {c \ zr ⁱⁿᵗ ir : 𝕍}, snd Ω)  M'
+        }> (ev <| env ; vars ::= fun e => e{c \VInt (zr ⁱⁿᵗ ir) : 𝕍} |> <| mstate := M |> )
     ). {
-    exists M{lr\Defined zr,l2\Defined z2,l1\Defined z1}. intros H2 [H3 H4].  apply S_Seq with Ω M{l1\Defined z1}. 
+    exists ev.(mstate){lr\Defined zr,l2\Defined z2,l1\Defined z1}. intros H2 [H3 H4].  apply S_Seq with (ev <| mstate ::= {{l1\Defined z1}} |>). 
     - apply semantics_of_the_mpz_assgn_macro...
-    - apply S_Seq with Ω M{l2\Defined z2,l1\Defined z1}.
+    - apply S_Seq with (ev <| mstate ::= {{l1\Defined z1}} |> <| mstate ::= {{l2\Defined z2}} |> ). 
         + apply semantics_of_the_mpz_assgn_macro... apply same_eval_macro with v1...
-        + apply S_Seq with Ω M{lr\Defined zr,l2\Defined z2,l1\Defined z1}.
+        + apply S_Seq with (ev <| mstate ::= {{l1\Defined z1}} |> <| mstate ::= {{l2\Defined z2}}  |> <| mstate ::= {{lr\Defined zr}} |>).
             * constructor. apply S_op with l1 l2...
                 ** constructor... easy. apply GMP_E_Var with z1... destruct (eq_dec l1 l2).
                     *** subst. edestruct Hnoalias...
-                    *** apply p_map_not_same_eq...
+                    *** apply p_map_not_same_eq... autounfold with rac_hint. simpl...
                 ** destruct (eq_dec l1 l2).
                     *** subst. edestruct Hnoalias...
-                    *** apply p_map_not_same_eq...
-                ** constructor... easy.
-            * apply semantics_of_the_int_assgn_macro...  apply M_Mpz with lr...
-                constructor... easy. 
+                    *** apply p_map_not_same_eq...  autounfold with rac_hint. simpl...
+                ** constructor... easy. constructor 1 with z2. simpl... autounfold with rac_hint. simpl...
+                ** simpl...
+            * replace (ev <| env; vars ::= _ |> <| mstate :=  _ |>)
+            with (ev <| mstate := ev.(mstate) {lr \Defined zr, l2 \Defined z2, l1 \ Defined z1} |> 
+                    <| env; vars ::= {{c \Def (VInt ((zr ⁱⁿᵗ) ir))}} |>
+            ) by reflexivity.
+            apply semantics_of_the_int_assgn_macro...  apply M_Mpz with lr ; simpl...
+                constructor... easy. constructor 1 with zr ; simpl...
     }
     
     unfold binop_ASSGN. destruct (ty e1) eqn:T1, (ty e2) eqn:T2 ; try apply NotInt. clear NotInt.
-    exists M. intros. inversion H0 ; inversion H1; try 
+    exists ev.(mstate). intros. inversion H0 ; inversion H1; try 
     match goal with 
-    | Contra :  (_ ⋅ _ |= _ => Def (VMpz _))%gmpsem |- _ => 
+    | Contra :  ( _ |= _ => Def (VMpz _))%gmpesem |- _ => 
         inversion Contra ; match goal with 
-        | Contra : _gmp_exp_sem _ _ _ _ |- _ => inversion Contra ; now subst
+        | Contra : _gmp_exp_sem _ _ _ |- _ => inversion Contra ; now subst
         end
     end.
     - subst. constructor... destruct x,x0. econstructor...
@@ -1112,30 +1113,37 @@ Qed.
 
 
 Lemma semantics_of_the_binop_macro_mpz :
-    forall funs procs (Ω:Ω) (M:𝓜) (op:fsl_binop_int) c y r e1 e2 v1 v2 z1 z2 l1 l2,
-    _no_env_mpz_aliasing Ω ->
-    type_of_value ((fst Ω) c) = Some C_Int ->
-    Ω ⋅ M |= e1 ⇝ z1 ->
-    Ω ⋅ M |= e2 ⇝ z2 ->
+    forall funs procs (ev:Env) (op:fsl_binop_int) c y r e1 e2 v1 v2 z1 z2 l1 l2,
+    _no_env_mpz_aliasing ev ->
+    type_of_value (ev c) = Some C_Int ->
+    ev |= e1 ⇝ z1 ->
+    ev |= e2 ⇝ z2 ->
 
-    let zr := ⋄ (□ op) z1 z2 in
-    (fst Ω) v1 = Some (Def (VMpz (Some l1))) /\  (fst Ω) v2 = Some (Def (VMpz (Some l2))) /\  (fst Ω) c = Some (Def (VMpz (Some y))) ->
+    let zr := ⋄ op z1 z2 in
+    ev v1 = Some (Def (VMpz (Some l1))) /\  ev v2 = Some (Def (VMpz (Some l2))) /\  ev c = Some (Def (VMpz (Some y))) ->
     ~ List.In v1 (exp_vars e2) -> (* not in paper proof *)
-    exists M', (forall v n, (fst Ω) v = Some (Def (VMpz (Some n))) ->
-    ~ ((fst Ω) v1 = (fst Ω) v) /\ ~ ((fst Ω) v2 = (fst Ω) v)  -> M n = M' n) -> 
+    exists M, (forall v n, ev v = Some (Def (VMpz (Some n))) ->
+    ev v1 <> ev v /\ ev v2 <> ev v -> ev.(mstate) n = M n) -> 
     l1 <> l2 -> (* not in paper proof *)
-    gmp_stmt_sem funs procs Ω M (binop_ASSGN op (T_Ext Mpz,c) e1 e2 r v1 v2) Ω  M'{y\Defined zr}
+    gmp_stmt_sem funs procs ev (binop_ASSGN op (T_Ext Mpz,c) e1 e2 r v1 v2) (ev <| mstate := M{y\Defined zr} |>)
     .
 Proof with eauto using p_map_same with rac_hint.
-    intros funs procs Ω M op c y r e1 e2 v1 v2 z1 z2 l1 l2 Hnoalias H H0 H1 zr H2 H3. exists M{l2\Defined z2,l1\Defined z1}. intros. destruct H2 as (v1l & v2l & rl). unfold binop_ASSGN.
-    apply S_Seq with Ω M{l1\Defined z1}.
+    intros funs procs ev op c y r e1 e2 v1 v2 z1 z2 l1 l2 Hnoalias H H0 H1 zr H2 H3. 
+    exists ev.(mstate){l2\Defined z2,l1\Defined z1}. intros. destruct H2 as (v1l & v2l & rl). unfold binop_ASSGN.
+    apply S_Seq with (ev <| mstate ::= {{l1\Defined z1}} |>).
     - apply semantics_of_the_mpz_assgn_macro...
-    - apply S_Seq with Ω M{l2\Defined z2,l1\Defined z1}. 
+    - apply S_Seq with (ev <| mstate ::= {{l1\Defined z1}} |> <| mstate ::= {{l2\Defined z2}} |>). 
         * apply semantics_of_the_mpz_assgn_macro... apply same_eval_macro with v1...
-        * constructor. pose proof (p_map_not_same M{l1 \Defined z1}) l1 l2 z2 H5. simpl. apply S_op with l1 l2...
-            + constructor... easy. apply GMP_E_Var with z1... rewrite H2...
-            + rewrite H2...
-            + constructor... easy.
+        * constructor.  
+            replace  (ev <| mstate := ev.(mstate) {y \Defined zr, l2 \Defined z2, l1 \Defined z1} |>)
+            with (ev <| mstate ::= {{l1 \Defined z1}} |> 
+                    <| mstate ::= {{l2 \Defined z2}} |>
+                    <| mstate ::= {{y \Defined zr}} |> 
+            ) by reflexivity.
+        apply S_op with l1 l2 ; simpl...
+            + constructor... easy. apply GMP_E_Var with z1... simpl. apply p_map_not_same_eq...
+            + simpl. apply p_map_not_same_eq...
+            + constructor... easy. constructor 1 with z2... simpl...
 Qed.
 
 (* Preservation of the semantics *)
