Arithmetic/theories/Notations.v
@@ -9,7 +9,7 @@ Delimit Scope utils_scope with utils.
 
 Declare Custom Entry pmap.
 
-Notation "X ⇀ Y" :=  (X -> option Y) (at level 100): type_scope.
+Reserved Notation "X ⇀ Y"  (at level 100).
 Notation "A ⃰" := (list A) (at level 20) : type_scope.
 Notation "x '\' y" := (x,y) (in custom pmap at level 0, x constr, y constr) : utils_scope.
 Notation id := string.
@@ -17,10 +17,10 @@ Notation id := string.
 Reserved Notation "⊥".
 Reserved Notation "'dom' f" (at level 10).
 Reserved Notation "f { xy , .. , xy' }" (xy custom pmap, xy' custom pmap, at level 0).
-Reserved Notation "Ω |= e => v" (at level 70). (* semantic of expressions, v ∈ Value *)
-Reserved Notation "Ω ⋅ M |= e => v" (at level 70,  M at next level).  (* semantic of gmp expressions *) 
-Reserved Notation "Ω ⋅ M |= s => Ω' ⋅  M'" (at level 70,  M at next level, Ω' at next level).  (* semantic of statements *) 
-Reserved Notation "Ω ⋅ M '|=' e ⇝ z" (M at next level, at level 70).
+Reserved Notation "{{ xy , .. , xy' }}" (xy custom pmap, xy' custom pmap, at level 0).
+Reserved Notation "env |= e => v" (at level 70). (* semantic of expressions, v ∈ Value *)
+Reserved Notation "env |= s => env'" (at level 70,  env' at next level).  (* semantic of statements *) 
+Reserved Notation "env '|=' e ⇝ z" (at level 70).
 Reserved Notation "e ⊑ e'" ( e  constr, e'  constr, at level 99).
 Reserved Notation "( e , m ) ⊑ ( e' , m' )".
 Reserved Notation "e ⊑ e'" (at level 99).
